dafny/ver/L1/distr_system_spec/distributed_system.dfy
@@ -92,5 +92,2556 @@ module L1_DistributedSystem
                     DSNextNode(s, s', messagesSentByTheNodes, messagesReceivedByTheNodes, node)
             )
     }
+
+    function filterA<T>(
+        s: seq<T>,
+        seqNodes: seq<Address>,
+        node: Address     
+    ): seq<T>
+    requires |seqNodes| == |s|
+    {
+        if s == [] then 
+            []
+        else 
+            (
+                if seqNodes[0] == node then
+                    [s[0]] + filterA(s[1..], seqNodes[1..], node)
+                else
+                    []
+            )
+            + filterA(s[1..], seqNodes[1..], node)
+    }   
+
+    // function filterB(
+    //     seqMessagesSentByTheNodes: seq<set<QbftMessageWithRecipient>>,
+    //     seqNodes: seq<Address>,
+    //     node: Address     
+    // ): seq<set<QbftMessageWithRecipient>>
+    // requires |seqNodes| == |seqMessagesSentByTheNodes| > 0
+    // {
+    //     if seqNodes == [] then 
+    //         []
+    //     else 
+    //         (
+    //             if seqNodes[0] == node then
+    //                 [seqMessagesSentByTheNodes[0]] + filterA(seqMessagesSentByTheNodes[1..], seqNodes[1..], node)
+    //             else
+    //                 []
+    //         )
+    //         + filterA(seqMessagesSentByTheNodes[1..], seqNodes[1..], node)
+    // }   
+
+
+
+
+    // function QbftSpecificationBuilder(
+    //     configuration: Configuration,
+    //     id: Address
+    // ): QbftSpecification
+    // {
+    //     var behaviours:=
+    //         iset QbftNodeBehaviour: QbftNodeBehaviour |
+    //             exists nt: iseq<NodeState> ::
+    //                 && NodeInit(nt[0], configuration, id)
+    //                 && QbftNodeBehaviour.initialBlockchain == nt[0].blockchain
+    //                 && (forall i:nat ::
+    //                         (
+    //                             IsValidQbftBehaviourStep(QbftNodeBehaviour, nt ,i)
+    //                         //     var step := QbftNodeBehaviour.steps[i];
+    //                         //     && validNodeState(nt[i])
+    //                         // // && NodeNext(nt[i], step.messageReceived, nt[i+1], step.messagesToSend)
+    //                         // && step.newBlockchain == nt[i+1].blockchain
+    //                         )
+    //                 )
+    //         ;
+
+    //     QbftSpecification(behaviours)
+    // }  
+
+    datatype AdversarySpecificationStep = AdversarySpecificationStep(
+        messageReceived: set<QbftMessage>,
+        messagesToSend: set<QbftMessageWithRecipient>
+    )
+
+    datatype AdvesarySpecificationBehaviour = AdvesarySpecificationBehaviour(
+        steps: iseq<AdversarySpecificationStep>
+    )
+
+    datatype AdversarySpecification = AdversarySpecification(
+        behaviours: iset<AdvesarySpecificationBehaviour>
+    )
+
+    function AdversarySpecificationBuilder(
+        configuration: Configuration,
+        byzNodes: set<Address>
+    ): AdversarySpecification
+    {
+        var behaviours:=
+            iset advesarySpecificationBehaviour: AdvesarySpecificationBehaviour |
+                exists nt: iseq<Adversary> ::
+                    && AdversaryInit(nt[0], configuration)
+                    && nt[0].byz == byzNodes
+                    && (forall i:nat ::
+                            var step := advesarySpecificationBehaviour.steps[i];
+                            && AdversaryNext(nt[i], step.messageReceived, nt[i+1], step.messagesToSend)
+                    )
+            ;
+
+        AdversarySpecification(behaviours)
+    }  
+
+    datatype EnvironmentSpecificationStep = EnvironmentSpecificationStep(
+        messagesSentByTheNodes: set<QbftMessageWithRecipient>,
+        messagesReceivedByTheNodes: multiset<QbftMessageWithRecipient>
+    )
+
+    datatype EnvironmentSpecificationBehaviour = EnvironmentSpecificationBehaviour(
+        steps: iseq<EnvironmentSpecificationStep>
+    )
+
+    datatype EnvironmentSpecification = EnvironmentSpecification(
+        behaviours: iset<EnvironmentSpecificationBehaviour>
+    )    
+
+    function EnvironmentSpecificationBuilder(
+        configuration: Configuration
+    ): EnvironmentSpecification
+    {
+        var behaviours:=
+            iset environmentSpecificationBehaviour: EnvironmentSpecificationBehaviour |
+                exists nt: iseq<Network> ::
+                    && NetworkInit(nt[0], configuration)
+                    && (forall i:nat ::
+                            var step := environmentSpecificationBehaviour.steps[i];
+                            && NetworkNext(nt[i], nt[i+1], step.messagesSentByTheNodes, step.messagesReceivedByTheNodes)
+                    )
+            ;
+
+        EnvironmentSpecification(behaviours)
+    }      
+
+
+
+    datatype DSBehaviour = DSBehaviour(
+        nodesBehaviours: map<Address, QbftNodeBehaviour>,
+        adversaryBehaviour: AdvesarySpecificationBehaviour,
+        environmentBehaviour: EnvironmentSpecificationBehaviour
+    )
+
+    datatype DSSepcification = DSSepcification(
+        behaviours: iset<DSBehaviour>
+    )
+
+    predicate DSSpecificationBuilderHelper(
+        dsBehaviour: DSBehaviour,
+        allNodes: set<Address>,
+        seqNodes: iseq<Address>,
+        i: nat
+    )
+    {
+        var honestNodes := dsBehaviour.nodesBehaviours.Keys;
+        var environmentStep := dsBehaviour.environmentBehaviour.steps[i];
+        var node := seqNodes[i];
+        var messagesReceivedWithoutRecipient := (set mr:QbftMessageWithRecipient | mr in environmentStep.messagesReceivedByTheNodes :: mr.message);
+        var byz := allNodes - honestNodes;
+        && node in allNodes
+        && (forall mr:QbftMessageWithRecipient | mr in environmentStep.messagesReceivedByTheNodes :: mr.recipient == node)                        
+        &&  if node in honestNodes then
+                var stepsTakeByNodeSoFar := getStepsTakeByNodeSoFar(seqNodes, node, i);
+                var nodeStep := dsBehaviour.nodesBehaviours[node].steps[stepsTakeByNodeSoFar];
+                && nodeStep.messagesToSend == environmentStep.messagesSentByTheNodes
+                && nodeStep.messagesReceived == messagesReceivedWithoutRecipient
+            else 
+                var stepsTakeByNodeSoFar := getStepsTakeByAversarySoFar(seqNodes, byz, i);
+                var nodeStep := dsBehaviour.adversaryBehaviour.steps[stepsTakeByNodeSoFar];
+                && nodeStep.messagesToSend == environmentStep.messagesSentByTheNodes
+                && nodeStep.messageReceived == messagesReceivedWithoutRecipient
+    }
+
+    function DSSpecificationBuilder(
+        configuration: Configuration
+    ): DSSepcification 
+    requires IsValidConfiguration(configuration)
+    {
+        var allNodes := seqToSet(configuration.nodes);
+        var behaviours := 
+            iset dsBehaviour: DSBehaviour |
+                var honestNodes := dsBehaviour.nodesBehaviours.Keys;
+                var byzNodes := allNodes - honestNodes;
+                && honestNodes <= allNodes         
+                && |byzNodes| <= f(|validators([configuration.genesisBlock])|)         
+                && dsBehaviour.environmentBehaviour in EnvironmentSpecificationBuilder(configuration).behaviours
+                && dsBehaviour.adversaryBehaviour in AdversarySpecificationBuilder(configuration, byzNodes).behaviours
+                && (forall n | n in honestNodes :: IsValidQbftBehaviour(configuration, n, dsBehaviour.nodesBehaviours[n]))
+                // && (forall )
+                && exists seqNodes: iseq<Address> ::
+                    && forall i: nat ::
+                        DSSpecificationBuilderHelper(dsBehaviour, allNodes, seqNodes, i)
+                        // var environmentStep := dsBehaviour.environmentBehaviour.steps[i];
+                        // var node := seqNodes[i];
+                        // var stepsTakeByNodeSoFar := getStepsTakeByNodeSoFar(seqNodes, node, i);
+                        // var messagesReceivedWithoutRecipient := (set mr:QbftMessageWithRecipient | mr in environmentStep.messagesReceivedByTheNodes :: mr.message);
+                        // && node in allNodes
+                        // && (forall mr:QbftMessageWithRecipient | mr in environmentStep.messagesReceivedByTheNodes :: mr.recipient == node)                        
+                        // &&  if node in honestNodes then
+                        //         var nodeStep := dsBehaviour.nodesBehaviours[node].steps[stepsTakeByNodeSoFar];
+                        //         && nodeStep.messagesToSend == environmentStep.messagesSentByTheNodes
+                        //         && nodeStep.messageReceived == messagesReceivedWithoutRecipient
+                        //     else 
+                        //         var nodeStep := dsBehaviour.adversaryBehaviour.steps[stepsTakeByNodeSoFar];
+                        //         && nodeStep.messagesToSend == environmentStep.messagesSentByTheNodes
+                        //         && nodeStep.messageReceived == messagesReceivedWithoutRecipient
+            ;
+
+        DSSepcification(behaviours)
+    }
+
+    lemma lemmajkfladjklfaHelper(
+        QbftNodeBehaviour: QbftNodeBehaviour,
+        configuration: Configuration,
+        id: Address        
+    )
+    requires IsValidQbftBehaviour(configuration, id, QbftNodeBehaviour)
+    {
+        var nt: iseq<NodeState> :|
+                    && NodeInit(nt[0], configuration, id)
+                    && QbftNodeBehaviour.initialBlockchain == nt[0].blockchain
+                    && (forall i:nat ::
+                            (
+                                IsValidQbftBehaviourStep(QbftNodeBehaviour, nt ,i)
+                                // var step := QbftNodeBehaviour.steps[i];
+                                // && validNodeState(nt[i])
+                                // && NodeNext(nt[i], step.messageReceived, nt[i+1], step.messagesToSend)
+                                // && step.newBlockchain == nt[i+1].blockchain
+                            )
+                    )
+            ;
+    }
+
+    function getDummySeqNodes(
+        configuration: Configuration,
+        id: Address
+    ): (ret: iseq<NodeState>)
+    requires  |validators([configuration.genesisBlock])| > 0
+    ensures NodeInit(ret[0], configuration, id)
+    {
+        var nt: iseq<NodeState> := 
+            imap i: nat :: 
+                var ns: NodeState := NodeState(
+                    [configuration.genesisBlock],
+                    0,
+                    0,
+                    id,
+                    configuration,
+                    {},
+                    None,
+                    None,
+                    None,
+                    0
+                );
+                assert NodeInit(ns, configuration, id);
+                ns
+            ;
+        nt
+    }
+
+    // function getSeqHonestNodeStates(
+    //     nodeStates: iseq<NodeState>,
+    //     id: Address,
+    //     i: nat,
+    //     seqNodes: iseq<Address>
+    // ): nat
+    // {
+    //     if i == 0 then
+    //         (nodeStates[0], 0)
+    //     else
+    //         var prev := getSeqHonestNodeStates(nodeStates, id, i-1, seqNodes);
+    //         var stateIndex := 
+    //             if id == seqNodes[i-1] then
+    //                 prev.1+1
+    //             else
+    //                 prev.1
+    //             ;
+    //         (prev + [nodeStates[stateIndex]], stateIndex)
+
+    // }
+
+    predicate pLemmajkfladjklfaGetSeqNodes(
+       dsBehaviour: DSBehaviour,
+       allNodes: set<Address>,
+       seqNodes: iseq<Address>
+    )
+    {
+        && (forall i: nat :: DSSpecificationBuilderHelper(dsBehaviour, allNodes, seqNodes, i))
+        && (forall i: nat :: seqNodes[i] in allNodes)
+    }
+
+
+    lemma lemmajkfladjklfaGetSeqNodes (
+       dsBehaviour: DSBehaviour,
+       configuration: Configuration,
+       allNodes: set<Address>
+    ) returns (seqNodes: iseq<Address>)
+    requires IsValidConfiguration(configuration)
+    requires dsBehaviour in DSSpecificationBuilder(configuration).behaviours
+    requires  |validators([configuration.genesisBlock])| > 0
+    requires allNodes == seqToSet(configuration.nodes);
+    ensures pLemmajkfladjklfaGetSeqNodes(dsBehaviour, allNodes, seqNodes)
+    {
+        seqNodes :|
+            && forall i: nat ::
+                DSSpecificationBuilderHelper(dsBehaviour, allNodes, seqNodes, i)
+            ;   
+
+        forall i: nat 
+        ensures seqNodes[i] in allNodes;
+        {
+            assert  DSSpecificationBuilderHelper(dsBehaviour, allNodes, seqNodes, i);
+            assert seqNodes[i] in allNodes;
+        }     
+    }
+
+    predicate pLemmajkfladjklfaGetAdvStatesHelper(
+        dsBehaviour: DSBehaviour,
+        seqAdvStates: iseq<Adversary>,
+        i: nat
+    )
+    {
+        var step := dsBehaviour.adversaryBehaviour.steps[i];
+        && AdversaryNext(seqAdvStates[i], step.messageReceived, seqAdvStates[i+1], step.messagesToSend)        
+    }
+
+    lemma lemmajkfladjklfaGetAdvStatesHelper(
+       dsBehaviour: DSBehaviour,
+       configuration: Configuration,
+       allNodes: set<Address>
+    ) returns (seqAdvStates: iseq<Adversary>)
+    requires IsValidConfiguration(configuration)
+    requires dsBehaviour in DSSpecificationBuilder(configuration).behaviours
+    requires  |validators([configuration.genesisBlock])| > 0
+    requires allNodes == seqToSet(configuration.nodes);
+    ensures && AdversaryInit(seqAdvStates[0], configuration)
+            && (forall i:nat ::
+                    pLemmajkfladjklfaGetAdvStatesHelper(dsBehaviour, seqAdvStates, i)
+                    // var step := dsBehaviour.adversaryBehaviour.steps[i];
+                    // && AdversaryNext(seqAdvStates[i], step.messageReceived, seqAdvStates[i+1], step.messagesToSend)
+            )
+        ;   
+    ensures seqAdvStates[0].byz == allNodes - dsBehaviour.nodesBehaviours.Keys     
+    {
+        var byz := allNodes - dsBehaviour.nodesBehaviours.Keys;
+        seqAdvStates :| 
+            && AdversaryInit(seqAdvStates[0], configuration)
+            && seqAdvStates[0].byz == byz
+            && (forall i:nat ::
+                    var step := dsBehaviour.adversaryBehaviour.steps[i];
+                    && AdversaryNext(seqAdvStates[i], step.messageReceived, seqAdvStates[i+1], step.messagesToSend)
+            )
+        ;           
+    }
+
+    lemma lemmajkfladjklfaGetAdvStatesHelper2(
+        dsBehaviour: DSBehaviour,
+        configuration: Configuration,
+        allNodes: set<Address>,
+        seqNodes: iseq<Address>,
+        seqAdvStatesOrig: iseq<Adversary>,
+        seqAdvStates: iseq<Adversary>  
+    ) 
+    requires IsValidConfiguration(configuration)
+    requires dsBehaviour in DSSpecificationBuilder(configuration).behaviours
+    requires  |validators([configuration.genesisBlock])| > 0
+    requires allNodes == seqToSet(configuration.nodes);
+    requires && AdversaryInit(seqAdvStatesOrig[0], configuration)
+            && (forall i:nat ::
+                    pLemmajkfladjklfaGetAdvStatesHelper(dsBehaviour, seqAdvStatesOrig, i)
+                    // var step := dsBehaviour.adversaryBehaviour.steps[i];
+                    // && AdversaryNext(seqAdvStates[i], step.messageReceived, seqAdvStates[i+1], step.messagesToSend)
+            )
+        ;        
+    requires
+            var byz := allNodes - dsBehaviour.nodesBehaviours.Keys;  
+            seqAdvStates ==   
+                imap i: nat :: 
+                    var stepsTakeByNodeSoFar := getStepsTakeByAversarySoFar(seqNodes, byz, i);
+                    seqAdvStatesOrig[stepsTakeByNodeSoFar];
+    ensures && AdversaryInit(seqAdvStates[0], configuration)
+    ensures 
+                var byz := allNodes - dsBehaviour.nodesBehaviours.Keys;
+                var adversarySpecificationBehaviour := dsBehaviour.adversaryBehaviour;
+            forall i: nat ::
+                if seqNodes[i] in byz then
+                    var stepsTakenByNodeSoFar := getStepsTakeByAversarySoFar(seqNodes, byz, i);
+                    var step := adversarySpecificationBehaviour.steps[stepsTakenByNodeSoFar];
+                    AdversaryNext(seqAdvStates[i], step.messageReceived, seqAdvStates[i+1], step.messagesToSend)
+                else
+                    seqAdvStates[i] == seqAdvStates[i+1];  
+
+    // ensures seqAdvStates[0].byz == allNodes - dsBehaviour.nodesBehaviours.Keys   
+    {
+
+        var byz := allNodes - dsBehaviour.nodesBehaviours.Keys;
+        var adversarySpecificationBehaviour := dsBehaviour.adversaryBehaviour;
+
+        forall i: nat 
+        ensures
+            if seqNodes[i] in byz then
+                var stepsTakenByNodeSoFar := getStepsTakeByAversarySoFar(seqNodes, byz, i);
+                var step := adversarySpecificationBehaviour.steps[stepsTakenByNodeSoFar];
+                AdversaryNext(seqAdvStates[i], step.messageReceived, seqAdvStates[i+1], step.messagesToSend)
+            else
+                seqAdvStates[i] == seqAdvStates[i+1];
+        {
+            lemmaGetStepsTakeByAdversarySoFar(seqNodes, byz, i);
+            if seqNodes[i] in byz 
+            {
+                var stepsTakenByNodeSoFar := getStepsTakeByAversarySoFar(seqNodes, byz, i);
+                assert getStepsTakeByAversarySoFar(seqNodes, byz, i + 1) == stepsTakenByNodeSoFar + 1;
+
+                assert seqAdvStates[i] == seqAdvStatesOrig[stepsTakenByNodeSoFar];
+                assert seqAdvStates[i+1] == seqAdvStatesOrig[stepsTakenByNodeSoFar+1];
+
+                // lemmaGetSeqHonestNodeStatesHelper(QbftNodeBehaviour, nt, stepsTakenByNodeSoFar);
+
+                // // assert IsValidQbftBehaviourStep(QbftNodeBehaviour, nt ,stepsTakenByNodeSoFar);
+                // assert validNodeState(seqNodeStates[i]); 
+                // assert validNodeState(nt[stepsTakenByNodeSoFar]); 
+                var step := adversarySpecificationBehaviour.steps[stepsTakenByNodeSoFar];
+                assert pLemmajkfladjklfaGetAdvStatesHelper(dsBehaviour, seqAdvStatesOrig, stepsTakenByNodeSoFar);
+                assert AdversaryNext(seqAdvStatesOrig[stepsTakenByNodeSoFar], step.messageReceived, seqAdvStatesOrig[stepsTakenByNodeSoFar+1], step.messagesToSend);
+                assert AdversaryNext(seqAdvStates[i], step.messageReceived, seqAdvStates[i+1], step.messagesToSend);
+                // assert NodeNext(nt[stepsTakenByNodeSoFar], step.messageReceived, nt[stepsTakenByNodeSoFar+1], step.messagesToSend);
+                // assert NodeNext(seqNodeStates[i], step.messageReceived, seqNodeStates[i+1], step.messagesToSend);
+            }
+            else
+            {
+                assert seqAdvStates[i] == seqAdvStates[i+1];
+            }
+        }        
+    }
+
+
+    lemma lemmajkfladjklfaGetAdvStates(
+       dsBehaviour: DSBehaviour,
+       configuration: Configuration,
+       allNodes: set<Address>,
+       seqNodes: iseq<Address>
+    ) returns (seqAdvStates: iseq<Adversary>)
+    requires IsValidConfiguration(configuration)
+    requires dsBehaviour in DSSpecificationBuilder(configuration).behaviours
+    requires  |validators([configuration.genesisBlock])| > 0
+    requires allNodes == seqToSet(configuration.nodes);
+    // ensures && AdversaryInit(seqAdvStates[0], configuration)
+    //         && (forall i:nat ::
+    //                 var step := dsBehaviour.adversaryBehaviour.steps[i];
+    //                 && AdversaryNext(seqAdvStates[i], step.messageReceived, seqAdvStates[i+1], step.messagesToSend)
+    //         )
+    //     ;   
+    ensures seqAdvStates[0].byz == allNodes - dsBehaviour.nodesBehaviours.Keys 
+    ensures forall i: nat ::  seqAdvStates[0].byz == seqAdvStates[i].byz
+    ensures AdversaryInit(seqAdvStates[0], configuration)
+    ensures 
+        var adversarySpecificationBehaviour := dsBehaviour.adversaryBehaviour;
+        var byz := allNodes - dsBehaviour.nodesBehaviours.Keys;
+        forall i: nat ::
+            if seqNodes[i] in byz then
+                var stepsTakenByNodeSoFar := getStepsTakeByAversarySoFar(seqNodes, byz, i);
+                var step := adversarySpecificationBehaviour.steps[stepsTakenByNodeSoFar];
+                AdversaryNext(seqAdvStates[i], step.messageReceived, seqAdvStates[i+1], step.messagesToSend)
+            else
+                seqAdvStates[i] == seqAdvStates[i+1];        
+    {      
+        var byz := allNodes - dsBehaviour.nodesBehaviours.Keys;
+        var seqAdvStatesOrig := lemmajkfladjklfaGetAdvStatesHelper(dsBehaviour, configuration, allNodes);
+        // var seqAdvStatesOrig: iseq<Adversary> :| 
+        //     && AdversaryInit(seqAdvStatesOrig[0], configuration)
+        //     && seqAdvStatesOrig[0].byz == byz
+        //     && (forall i:nat ::
+        //             var step := dsBehaviour.adversaryBehaviour.steps[i];
+        //             && AdversaryNext(seqAdvStatesOrig[i], step.messageReceived, seqAdvStatesOrig[i+1], step.messagesToSend)
+        //     )
+        // ;    
+
+        assert seqAdvStatesOrig[0].byz == allNodes - dsBehaviour.nodesBehaviours.Keys;
+
+        seqAdvStates := 
+            imap i: nat :: 
+            var stepsTakeByNodeSoFar := getStepsTakeByAversarySoFar(seqNodes, byz, i);
+            seqAdvStatesOrig[stepsTakeByNodeSoFar];
+
+        var adversarySpecificationBehaviour := dsBehaviour.adversaryBehaviour;
+
+        forall i: nat 
+        ensures
+            if seqNodes[i] in byz then
+                var stepsTakenByNodeSoFar := getStepsTakeByAversarySoFar(seqNodes, byz, i);
+                var step := adversarySpecificationBehaviour.steps[stepsTakenByNodeSoFar];
+                AdversaryNext(seqAdvStates[i], step.messageReceived, seqAdvStates[i+1], step.messagesToSend)
+            else
+                seqAdvStates[i] == seqAdvStates[i+1];
+        {
+            lemmajkfladjklfaGetAdvStatesHelper2(dsBehaviour, configuration, allNodes, seqNodes, seqAdvStatesOrig, seqAdvStates);
+        }
+
+        forall i: nat
+        ensures seqAdvStatesOrig[0].byz == seqAdvStatesOrig[i].byz
+        {
+            lemmajkfladjklfaGetDsStatesHelper(dsBehaviour, configuration, seqAdvStatesOrig, i);
+        }
+
+        assert forall i: nat :: seqAdvStates[0].byz == seqAdvStates[i].byz;
+    }
+
+    predicate lemmajkfladjklfaGetEnvStatesHelper(
+        seqEnvStates: iseq<Network>,
+        environmentSpecificationBehaviour: EnvironmentSpecificationBehaviour,
+        i: nat
+    )
+    {
+        var step := environmentSpecificationBehaviour.steps[i];
+        && NetworkNext(seqEnvStates[i], seqEnvStates[i+1], step.messagesSentByTheNodes, step.messagesReceivedByTheNodes)
+    }
+
+    lemma lemmajkfladjklfaGetEnvStates(
+       dsBehaviour: DSBehaviour,
+       configuration: Configuration
+    ) returns (seqEnvStates: iseq<Network>)
+    requires IsValidConfiguration(configuration)
+    requires dsBehaviour in DSSpecificationBuilder(configuration).behaviours
+    ensures     && NetworkInit(seqEnvStates[0], configuration)
+                && (forall i:nat ::
+                        lemmajkfladjklfaGetEnvStatesHelper(seqEnvStates, dsBehaviour.environmentBehaviour, i)
+                        // var step := dsBehaviour.environmentBehaviour.steps[i];
+                        // && NetworkNext(seqEnvStates[i], seqEnvStates[i+1], step.messagesSentByTheNodes, step.messagesReceivedByTheNodes)
+                )
+    {
+        seqEnvStates :|
+                && NetworkInit(seqEnvStates[0], configuration)
+                && (forall i:nat ::
+                        var step := dsBehaviour.environmentBehaviour.steps[i];
+                        && NetworkNext(seqEnvStates[i], seqEnvStates[i+1], step.messagesSentByTheNodes, step.messagesReceivedByTheNodes)
+                )
+        ;       
+         
+    }
+
+    function getStepsTakeByNodeSoFar(
+        seqNodes: iseq<Address>,
+        node: Address,
+        step: nat
+    ): nat 
+    {
+        var stepsTakenByNode :=
+            set i: nat |
+                && i < step 
+                && seqNodes[i] == node
+            ;
+
+        |stepsTakenByNode|
+    }
+
+    function getStepsTakeByAversarySoFar(
+        seqNodes: iseq<Address>,
+        byz: set<Address>,
+        step: nat
+    ): nat     
+    {
+        var stepsTakenByAdversary :=
+            set i: nat |
+                && i < step 
+                && seqNodes[i] in byz
+            ;
+
+        |stepsTakenByAdversary|        
+    }    
+
+
+    function getStepsTakeByNodeSoFarReverseHelper(
+        seqNodes: iseq<Address>,
+        node: Address,
+        ret: nat,
+        test: nat
+    ): (inv: nat)
+    requires getStepsTakeByNodeSoFar(seqNodes,node, test) >= ret 
+    ensures getStepsTakeByNodeSoFar(seqNodes, node, inv) == ret 
+    {
+        if getStepsTakeByNodeSoFar(seqNodes, node, test) == ret then 
+            test 
+        else
+            assert test > 0 by {
+                if test == 0 
+                {
+                    assert getStepsTakeByNodeSoFar(seqNodes, node, test) == 0;
+                    assert ret == 0;
+                    assert false;
+                }
+            }
+            var retTest := getStepsTakeByNodeSoFar(seqNodes, node, test);
+            assert retTest > 0;
+            var retTestMinusOne := getStepsTakeByNodeSoFar(seqNodes, node, test-1);
+            lemmaGetStepsTakeByNodeSoFar(seqNodes, node, test - 1);
+            assert retTest -1 <= retTestMinusOne <= retTest;
+
+            var inv := getStepsTakeByNodeSoFarReverseHelper(seqNodes, node, ret, test-1);
+            inv
+    }
+
+    // predicate pGetStepsTakeByNodeSoFarReversePrecondition(
+    //     seqNodes: iseq<Address>,
+    //     node: Address,
+    //     ret: nat
+    // ): (inv: nat)
+
+    function getStepsTakeByNodeSoFarReverse(
+        seqNodes: iseq<Address>,
+        node: Address,
+        ret: nat
+    ): (inv: nat)
+    requires exists bound: nat :: getStepsTakeByNodeSoFar(seqNodes,node, bound) >= ret
+    ensures getStepsTakeByNodeSoFar(seqNodes, node, inv) == ret 
+    {
+        var bound: nat :| getStepsTakeByNodeSoFar(seqNodes,node, bound) >= ret;
+        getStepsTakeByNodeSoFarReverseHelper(seqNodes, node, ret, bound)
+    }
+
+    lemma lemmaGetStepsTakeByNodeSoFar
+    (
+        seqNodes: iseq<Address>,
+        node: Address,
+        step: nat        
+    )
+    ensures 
+        if seqNodes[step] == node  then
+            getStepsTakeByNodeSoFar(seqNodes,node, step) + 1 == getStepsTakeByNodeSoFar(seqNodes, node, step +1)
+        else
+            getStepsTakeByNodeSoFar(seqNodes,node, step)  == getStepsTakeByNodeSoFar(seqNodes, node, step +1)
+
+    ensures getStepsTakeByNodeSoFar(seqNodes,node, step)  <= getStepsTakeByNodeSoFar(seqNodes, node, step +1)
+    {
+        assert getStepsTakeByNodeSoFar(seqNodes,node, 0) == 0;
+        var stepsTakenByNode :=
+            set i: nat |
+                && i < step 
+                && seqNodes[i] == node
+            ;
+
+        var stepsTakenByNodePlusOne :=
+            set i: nat |
+                && i < (step + 1)
+                && seqNodes[i] == node
+            ;   
+
+        
+        if seqNodes[step] == node 
+        {
+            assert step !in stepsTakenByNode;
+            assert stepsTakenByNodePlusOne == stepsTakenByNode + {step};
+            assert |stepsTakenByNode| + 1 == |stepsTakenByNodePlusOne|;
+            assert getStepsTakeByNodeSoFar(seqNodes,node, step) + 1 == getStepsTakeByNodeSoFar(seqNodes, node, step +1);
+        }
+        else
+        {
+            assert stepsTakenByNodePlusOne == stepsTakenByNode;
+            assert |stepsTakenByNode| == |stepsTakenByNodePlusOne|;
+            assert getStepsTakeByNodeSoFar(seqNodes,node, step)  == getStepsTakeByNodeSoFar(seqNodes, node, step +1);            
+        }
+    }
+
+    lemma lemmaGetStepsTakeByAdversarySoFar
+    (
+        seqNodes: iseq<Address>,
+        byz: set<Address>,
+        step: nat        
+    )
+    ensures 
+        if seqNodes[step] in byz  then
+            getStepsTakeByAversarySoFar(seqNodes, byz, step) + 1 == getStepsTakeByAversarySoFar(seqNodes, byz, step +1)
+        else
+            getStepsTakeByAversarySoFar(seqNodes, byz, step) == getStepsTakeByAversarySoFar(seqNodes, byz, step +1)
+    {
+        // assert getStepsTakeByNodeSoFar(seqNodes,node, 0) == 0;
+        var stepsTakenByNode :=
+            set i: nat |
+                && i < step 
+                && seqNodes[i] in byz
+            ;
+
+        var stepsTakenByNodePlusOne :=
+            set i: nat |
+                && i < (step + 1)
+                && seqNodes[i] in byz
+            ;   
+
+        
+        if seqNodes[step] in byz
+        {
+            assert step !in stepsTakenByNode;
+            assert stepsTakenByNodePlusOne == stepsTakenByNode + {step};
+            assert |stepsTakenByNode| + 1 == |stepsTakenByNodePlusOne|;
+            assert getStepsTakeByAversarySoFar(seqNodes, byz, step) + 1 == getStepsTakeByAversarySoFar(seqNodes, byz, step +1);
+        }
+        else
+        {
+            assert stepsTakenByNodePlusOne == stepsTakenByNode;
+            assert |stepsTakenByNode| == |stepsTakenByNodePlusOne|;
+            assert getStepsTakeByAversarySoFar(seqNodes, byz, step) == getStepsTakeByAversarySoFar(seqNodes, byz, step +1);      
+        }
+    }    
+
+    lemma lemmaGetSeqHonestNodeStatesHelper(
+        QbftNodeBehaviour: QbftNodeBehaviour,
+        nt: iseq<NodeState>,
+        i: nat
+    )
+    requires IsValidQbftBehaviourStep(QbftNodeBehaviour, nt ,i);
+    ensures validNodeState(nt[i])
+    ensures 
+                var step := QbftNodeBehaviour.steps[i];
+                NodeNext(nt[i], step.messagesReceived, nt[i+1], step.messagesToSend);
+    {  }
+
+    predicate pGetSeqHonestNodeStatesHelper(
+        QbftNodeBehaviour: QbftNodeBehaviour,
+        seqNodes: iseq<Address>,
+        seqNodeStates: iseq<NodeState>,
+        n: Address,
+        i: nat
+    )
+    {
+        if seqNodes[i] == n then 
+            var stepsTakenByNodeSoFar := getStepsTakeByNodeSoFar(seqNodes, n, i);
+            var step := QbftNodeBehaviour.steps[stepsTakenByNodeSoFar];
+            && validNodeState(seqNodeStates[i])
+            && NodeNext(seqNodeStates[i], step.messagesReceived, seqNodeStates[i+1], step.messagesToSend)
+            // && step.newBlockchain == seqNodeStates[i+1].blockchain
+        else
+            seqNodeStates[i] == seqNodeStates[i+1]        
+    }
+
+    // lemma lemmaHonestNodesAllValidsRecursive(
+    //     QbftNodeBehaviour: QbftNodeBehaviour,
+    //     nt: iseq<NodeState>,
+    //     configuration: Configuration,
+    //     n: Address,
+    //     i: nat
+    // )
+    // requires 
+    //         && NodeInit(nt[0], configuration, n)
+    //         && (forall i:nat ::
+    //                 IsValidQbftBehaviourStep(QbftNodeBehaviour, nt ,i)
+    //                 // var step := QbftNodeBehaviour.steps[i];
+    //                 // && validNodeState(nt[i])
+    //                 // && NodeNext(nt[i], step.messageReceived, nt[i+1], step.messagesToSend)
+    //                 // && step.newBlockchain == nt[i+1].blockchain
+    //         );      
+
+    // lemma lemmaHonestNodesAllValids(
+    //     QbftNodeBehaviour: QbftNodeBehaviour,
+    //     nt: iseq<NodeState>,
+    //     configuration: Configuration,
+    //     n: Address,
+    //     i: nat
+    // )
+    // requires 
+    //         && NodeInit(nt[0], configuration, n)
+    //         && (forall i:nat ::
+    //                 IsValidQbftBehaviourStep(QbftNodeBehaviour, nt ,i)
+    //                 // var step := QbftNodeBehaviour.steps[i];
+    //                 // && validNodeState(nt[i])
+    //                 // && NodeNext(nt[i], step.messageReceived, nt[i+1], step.messagesToSend)
+    //                 // && step.newBlockchain == nt[i+1].blockchain
+    //         );    
+    // {
+    //     if i == 0
+    //     {
+    //         assert validNodeState(nt[i]);
+    //     }
+    //     else
+    //     {
+    //         lemmaHonestNodesAllValidsRecursive(QbftNodeBehaviour, nt, configuration, n, i-1);
+
+    //     }
+    // }
+
+
+
+
+    lemma lemmaGetSeqHonestNodeStates2Helper(
+        dsBehaviour: DSBehaviour,
+        configuration: Configuration,       
+        n: Address,
+        seqNodes: iseq<Address>,
+        seqNodeStates: iseq<NodeState>
+    ) returns (nt: iseq<NodeState>)
+    requires n in dsBehaviour.nodesBehaviours
+    requires IsValidQbftBehaviour(configuration, n, dsBehaviour.nodesBehaviours[n])
+    // requires  |validators([configuration.genesisBlock])| > 0    
+    requires seqNodeStates == getSeqHonestNodeStates(dsBehaviour, configuration, n, seqNodes)    
+    ensures var QbftNodeBehaviour := dsBehaviour.nodesBehaviours[n];
+            && NodeInit(nt[0], configuration, n)
+            && QbftNodeBehaviour.initialBlockchain == nt[0].blockchain
+            && (forall i:nat ::
+                    IsValidQbftBehaviourStep(QbftNodeBehaviour, nt ,i)
+                    // var step := QbftNodeBehaviour.steps[i];
+                    // && validNodeState(nt[i])
+                    // && NodeNext(nt[i], step.messageReceived, nt[i+1], step.messagesToSend)
+                    // && step.newBlockchain == nt[i+1].blockchain
+            )
+            &&  seqNodeStates == 
+                imap i: nat :: 
+                    var stepsTakeByNodeSoFar := getStepsTakeByNodeSoFar(seqNodes, n, i);
+                    nt[stepsTakeByNodeSoFar] ;    
+    {
+        var QbftNodeBehaviour := dsBehaviour.nodesBehaviours[n];
+        nt :|
+            && NodeInit(nt[0], configuration, n)
+            && QbftNodeBehaviour.initialBlockchain == nt[0].blockchain
+            && (forall i:nat ::
+                    IsValidQbftBehaviourStep(QbftNodeBehaviour, nt ,i)
+                    // var step := QbftNodeBehaviour.steps[i];
+                    // && validNodeState(nt[i])
+                    // && NodeNext(nt[i], step.messageReceived, nt[i+1], step.messagesToSend)
+                    // && step.newBlockchain == nt[i+1].blockchain
+            )
+            &&  seqNodeStates == 
+                imap i: nat :: 
+                    var stepsTakeByNodeSoFar := getStepsTakeByNodeSoFar(seqNodes, n, i);
+                    nt[stepsTakeByNodeSoFar] ;         
+    }
+
+    lemma lemmaGetSeqHonestNodeStates2(
+        dsBehaviour: DSBehaviour,
+        configuration: Configuration,       
+        n: Address,
+        seqNodes: iseq<Address>,
+        seqNodeStates: iseq<NodeState>,
+        i: nat
+    )
+    requires n in dsBehaviour.nodesBehaviours
+    requires IsValidQbftBehaviour(configuration, n, dsBehaviour.nodesBehaviours[n])
+    requires  |validators([configuration.genesisBlock])| > 0    
+    requires seqNodeStates == getSeqHonestNodeStates(dsBehaviour, configuration, n, seqNodes)
+    ensures validNodeState(seqNodeStates[i]);
+    {
+        var QbftNodeBehaviour := dsBehaviour.nodesBehaviours[n];
+        lemmaGetSeqHonestNodeStates(dsBehaviour, configuration, n, seqNodes, seqNodeStates);
+        var nt := lemmaGetSeqHonestNodeStates2Helper(dsBehaviour, configuration, n, seqNodes, seqNodeStates);       
+        var j :| seqNodeStates[i] == nt[j];
+        assert IsValidQbftBehaviourStep(QbftNodeBehaviour, nt , j);
+        assert validNodeState(seqNodeStates[i]);
+    }
+
+
+
+    lemma lemmaGetSeqHonestNodeStates3Helepr(a: Blockchain, b: Blockchain, c: Blockchain)
+    requires a == b 
+    requires c == b
+    ensures a == c
+    ensures c == a
+    { }
+
+    lemma lemmaGetSeqHonestNodeStates3Helepr2(
+        seqNodes: iseq<Address>,
+        n: Address,
+        i: nat,
+        prevI: nat   
+    )
+    requires prevI == i - 1 
+    ensures getStepsTakeByNodeSoFar(seqNodes, n, prevI) == getStepsTakeByNodeSoFar(seqNodes, n, i-1);
+    {  }
+
+    lemma lemmaGetSeqHonestNodeStates3Helper3(
+        dsBehaviour: DSBehaviour,
+        configuration: Configuration,       
+        n: Address,
+        seqNodes: iseq<Address>,
+        seqNodeStates: iseq<NodeState>,
+        i: nat
+    )
+    requires n in dsBehaviour.nodesBehaviours
+    requires IsValidQbftBehaviour(configuration, n, dsBehaviour.nodesBehaviours[n])
+    requires  |validators([configuration.genesisBlock])| > 0    
+    requires seqNodeStates == getSeqHonestNodeStates(dsBehaviour, configuration, n, seqNodes) 
+    requires i > 0
+    requires getStepsTakeByNodeSoFar(seqNodes, n, i) == 0;  
+    ensures 
+            var QbftNodeBehaviour := dsBehaviour.nodesBehaviours[n];
+            seqNodeStates[i].blockchain ==  QbftNodeBehaviour.initialBlockchain;
+    decreases i,0
+    {
+        var QbftNodeBehaviour := dsBehaviour.nodesBehaviours[n];
+        var nt: iseq<NodeState> :|
+            && NodeInit(nt[0], configuration, n)
+            && QbftNodeBehaviour.initialBlockchain == nt[0].blockchain
+            && (forall i:nat ::
+                    IsValidQbftBehaviourStep(QbftNodeBehaviour, nt ,i)
+                    // var step := QbftNodeBehaviour.steps[i];
+                    // && validNodeState(nt[i])
+                    // && NodeNext(nt[i], step.messageReceived, nt[i+1], step.messagesToSend)
+                    // && step.newBlockchain == nt[i+1].blockchain
+            )
+            &&  seqNodeStates == 
+                imap i: nat :: 
+                    var stepsTakeByNodeSoFar := getStepsTakeByNodeSoFar(seqNodes, n, i);
+                    nt[stepsTakeByNodeSoFar] ;
+
+        var stpesTakenByTheNodeSoFar := getStepsTakeByNodeSoFar(seqNodes, n, i);
+        var prevI:nat := i-1;
+        lemmaGetSeqHonestNodeStates3(dsBehaviour, configuration, n, seqNodes, seqNodeStates, prevI);
+        lemmaGetSeqHonestNodeStates(dsBehaviour, configuration, n, seqNodes, seqNodeStates);
+
+        
+        var stpesTakenByTheNodeSoFarPrev := getStepsTakeByNodeSoFar(seqNodes, n, prevI);
+
+        lemmaGetStepsTakeByNodeSoFar(seqNodes, n, prevI);
+        assert stpesTakenByTheNodeSoFarPrev == 0;
+        var stepsTakenByNode :=
+            set j: nat |
+                && j <  i
+                && seqNodes[j] == n;
+
+        assert |stepsTakenByNode| == 0;   
+        assert stepsTakenByNode == {}; 
+
+        forall j: nat | j < i
+        ensures seqNodes[j] != n
+        {
+            if seqNodes[j] == n 
+            {
+                assert j in stepsTakenByNode;   
+                assert stepsTakenByNode != {};
+                assert false;
+            }
+
+            assert seqNodes[j] != n;
+        }
+
+        assert seqNodes[prevI] != n;
+        assert pGetSeqHonestNodeStatesHelper(QbftNodeBehaviour, seqNodes, seqNodeStates, n, prevI);
+        assert seqNodeStates[prevI] == seqNodeStates[prevI+1];
+        assert seqNodeStates[prevI] == seqNodeStates[i];
+        assert seqNodeStates[i].blockchain ==  QbftNodeBehaviour.initialBlockchain;                    
+    } 
+
+    lemma lemmaGetSeqHonestNodeStates3(
+        dsBehaviour: DSBehaviour,
+        configuration: Configuration,       
+        n: Address,
+        seqNodes: iseq<Address>,
+        seqNodeStates: iseq<NodeState>,
+        i: nat
+    )
+    requires n in dsBehaviour.nodesBehaviours
+    requires IsValidQbftBehaviour(configuration, n, dsBehaviour.nodesBehaviours[n])
+    requires  |validators([configuration.genesisBlock])| > 0    
+    requires seqNodeStates == getSeqHonestNodeStates(dsBehaviour, configuration, n, seqNodes)
+    ensures var QbftNodeBehaviour := dsBehaviour.nodesBehaviours[n];
+            var stpesTakenByTheNodeSoFar := getStepsTakeByNodeSoFar(seqNodes, n, i);
+            if stpesTakenByTheNodeSoFar == 0 then
+                seqNodeStates[i].blockchain ==  QbftNodeBehaviour.initialBlockchain
+            else
+                var stpesTakenByTheNodeSoFarPrev := stpesTakenByTheNodeSoFar - 1;
+                var step := QbftNodeBehaviour.steps[stpesTakenByTheNodeSoFarPrev];
+                seqNodeStates[i].blockchain == step.newBlockchain  
+    decreases i
+    {
+        var QbftNodeBehaviour := dsBehaviour.nodesBehaviours[n];
+        var nt: iseq<NodeState> :|
+            && NodeInit(nt[0], configuration, n)
+            && QbftNodeBehaviour.initialBlockchain == nt[0].blockchain
+            && (forall i:nat ::
+                    IsValidQbftBehaviourStep(QbftNodeBehaviour, nt ,i)
+                    // var step := QbftNodeBehaviour.steps[i];
+                    // && validNodeState(nt[i])
+                    // && NodeNext(nt[i], step.messageReceived, nt[i+1], step.messagesToSend)
+                    // && step.newBlockchain == nt[i+1].blockchain
+            )
+            &&  seqNodeStates == 
+                imap i: nat :: 
+                    var stepsTakeByNodeSoFar := getStepsTakeByNodeSoFar(seqNodes, n, i);
+                    nt[stepsTakeByNodeSoFar] ;
+
+        // if i == 0
+        // {
+        //     assert seqNodeStates[i].blockchain ==  QbftNodeBehaviour.initialBlockchain;
+        //         // assert seqNodeStates[i+1].blockchain == QbftNodeBehaviour.steps[getStepsTakeByNodeSoFar(seqNodes, n, i)].newBlockchain;            
+        // }
+        // else 
+        // {
+
+        // }
+
+
+        // var stpesTakenByTheNodeSoFar := getStepsTakeByNodeSoFar(seqNodes, n, i);
+
+        // lemmaGetSeqHonestNodeStates(dsBehaviour, configuration, n, seqNodes, seqNodeStates);
+        // assert pGetSeqHonestNodeStatesHelper(QbftNodeBehaviour, seqNodes, seqNodeStates, n, i);
+        // assert QbftNodeBehaviour.steps[i].newBlockchain == nt[getStepsTakeByNodeSoFar(seqNodes, n, i)+1].blockchain;
+
+        // assert stpesTakenByTheNodeSoFar > 0 ==> i > 0;
+        
+        var stpesTakenByTheNodeSoFar := getStepsTakeByNodeSoFar(seqNodes, n, i);
+        
+        if i == 0
+        {
+            assert seqNodeStates[i].blockchain ==  QbftNodeBehaviour.initialBlockchain;
+            assert stpesTakenByTheNodeSoFar == 0;
+                // assert seqNodeStates[i+1].blockchain == QbftNodeBehaviour.steps[getStepsTakeByNodeSoFar(seqNodes, n, i)].newBlockchain;            
+        }
+        else
+        {
+            var prevI:nat := i-1;
+            lemmaGetSeqHonestNodeStates3(dsBehaviour, configuration, n, seqNodes, seqNodeStates, prevI);
+            
+            var stpesTakenByTheNodeSoFarPrev := getStepsTakeByNodeSoFar(seqNodes, n, prevI);
+
+            lemmaGetStepsTakeByNodeSoFar(seqNodes, n, prevI);
+
+            if stpesTakenByTheNodeSoFar == 0
+            {
+                lemmaGetSeqHonestNodeStates3Helper3(dsBehaviour, configuration, n, seqNodes, seqNodeStates, i);
+                // assert stpesTakenByTheNodeSoFarPrev == 0;
+                // var stepsTakenByNode :=
+                //     set j: nat |
+                //         && j <  i
+                //         && seqNodes[j] == n;
+
+                // assert |stepsTakenByNode| == 0;   
+                // assert stepsTakenByNode == {}; 
+
+                // forall j: nat | j < i
+                // ensures seqNodes[j] != n
+                // {
+                //     if seqNodes[j] == n 
+                //     {
+                //         assert j in stepsTakenByNode;   
+                //         assert stepsTakenByNode != {};
+                //         assert false;
+                //     }
+
+                //     assert seqNodes[j] != n;
+                // }
+
+                // assert seqNodes[prevI] != n;
+                // assert seqNodeStates[i-1] == seqNodeStates[i];
+                // assert seqNodeStates[i].blockchain ==  QbftNodeBehaviour.initialBlockchain;
+                // assume seqNodeStates[i].blockchain ==  QbftNodeBehaviour.initialBlockchain;
+            }
+            else
+            {
+                if seqNodes[prevI] == n 
+                {
+                    calc == {
+                        getStepsTakeByNodeSoFar(seqNodes, n, prevI) + 1; 
+                        getStepsTakeByNodeSoFar(seqNodes, n, prevI+1);
+                        calc == {
+                            prevI + 1;
+                            i;
+                        }
+                        getStepsTakeByNodeSoFar(seqNodes, n, i);
+                    }
+                    assert stpesTakenByTheNodeSoFarPrev + 1 == stpesTakenByTheNodeSoFar;
+
+                    // var stepsTakenByNodeSoFar := getStepsTakeByNodeSoFar(seqNodes, n, i);
+                    assert seqNodeStates[i] == nt[stpesTakenByTheNodeSoFar];
+                    assert seqNodeStates[prevI] == nt[stpesTakenByTheNodeSoFarPrev];
+
+                    assert IsValidQbftBehaviourStep(QbftNodeBehaviour, nt, stpesTakenByTheNodeSoFarPrev); 
+
+                    // assert IsValidQbftBehaviourStep(QbftNodeBehaviour, nt, stpesTakenByTheNodeSoFar); 
+                    var prevStep := QbftNodeBehaviour.steps[prevI];
+                    // assert seqNodeStates[i].blockchain == prevStep.newBlockchain;
+                    // assert     
+                    // assert pGetSeqHonestNodeStatesHelper(QbftNodeBehaviour, seqNodes, seqNodeStates, n, prevI);
+                    var step := QbftNodeBehaviour.steps[stpesTakenByTheNodeSoFarPrev];
+                    var bc := nt[stpesTakenByTheNodeSoFarPrev+1].blockchain;
+                    assert step.newBlockchain ==  bc;
+                    assert seqNodeStates[i].blockchain == bc; // == step.newBlockchain;
+
+
+                    lemmaGetSeqHonestNodeStates3Helepr(step.newBlockchain, bc, seqNodeStates[i].blockchain);
+
+                    assert seqNodeStates[i].blockchain == step.newBlockchain;
+                    assert seqNodeStates[i].blockchain == QbftNodeBehaviour.steps[stpesTakenByTheNodeSoFarPrev].newBlockchain;
+
+                    assert seqNodeStates[i].blockchain == QbftNodeBehaviour.steps[getStepsTakeByNodeSoFar(seqNodes, n, i)-1].newBlockchain by 
+                    {
+                        calc == {
+                            seqNodeStates[i].blockchain; 
+                            QbftNodeBehaviour.steps[getStepsTakeByNodeSoFar(seqNodes, n, prevI)].newBlockchain;
+                            calc == {
+                                getStepsTakeByNodeSoFar(seqNodes, n, prevI);
+                                getStepsTakeByNodeSoFar(seqNodes, n, i) - 1;
+                            }
+                            QbftNodeBehaviour.steps[getStepsTakeByNodeSoFar(seqNodes, n, i)-1].newBlockchain;
+                        }
+                    }
+                }
+                else
+                {
+                    assert getStepsTakeByNodeSoFar(seqNodes, n, prevI) == getStepsTakeByNodeSoFar(seqNodes, n, prevI+1);
+                    assert seqNodeStates[prevI] == seqNodeStates[prevI+1] == seqNodeStates[i];
+
+                    assert seqNodeStates[i].blockchain == QbftNodeBehaviour.steps[getStepsTakeByNodeSoFar(seqNodes, n, i)-1].newBlockchain;
+                }
+            }
+        }
+        
+        
+
+        // forall i: nat 
+        // {
+        //         assert seqNodeStates[i].blockchain == nt[getStepsTakeByNodeSoFar(seqNodes, n, i)].blockchain;     
+
+        //         assert seqNodeStates[i+1].blockchain == QbftNodeBehaviour.steps[getStepsTakeByNodeSoFar(seqNodes, n, i)].newBlockchain;             
+        // }
+    } 
+
+    predicate pLemmaGetSeqHonestNodeStates4(
+        seqNodes: iseq<Address>,
+        n: Address,
+        j: nat, 
+        upperBound: nat
+    )
+    {
+        getStepsTakeByNodeSoFar(seqNodes, n, j) <= upperBound
+    }
+
+    predicate pLemmaGetSeqHonestNodeStates42(
+        seqNodes: iseq<Address>,
+        n: Address,
+        upperBound: nat
+    )
+    {
+        forall j: nat :: pLemmaGetSeqHonestNodeStates4(seqNodes, n, j, upperBound)
+    }    
+
+    predicate pGetStepsTakeByNodeSoFarIsLimited
+    (
+        seqNodes: iseq<Address>,
+        n: Address
+    )
+    {
+        exists max:nat :: pLemmaGetSeqHonestNodeStates42(seqNodes, n, max)
+    }
+
+    function getMaxWhenGetStepsTakeByNodeSoFarIsLimitedHelper
+    (
+        seqNodes: iseq<Address>,
+        n: Address,
+        test: nat
+    ) : (imaxAndMax: (nat, nat))
+    requires  pLemmaGetSeqHonestNodeStates42(seqNodes, n, test)
+    ensures getStepsTakeByNodeSoFar(seqNodes, n, imaxAndMax.0) == imaxAndMax.1;
+    ensures pLemmaGetSeqHonestNodeStates42(seqNodes, n, imaxAndMax.1)
+    {
+        if test == 0 then
+            var imaxAndMax := (0, 0);
+            assert getStepsTakeByNodeSoFar(seqNodes, n, imaxAndMax.0) == imaxAndMax.1;
+            imaxAndMax
+        
+        else
+        
+            if exists j: nat :: getStepsTakeByNodeSoFar(seqNodes, n, j) == test then
+            
+                var max := test;
+                var imax :| getStepsTakeByNodeSoFar(seqNodes, n, imax) == max;
+                var imaxAndMax := (imax, max);
+                assert getStepsTakeByNodeSoFar(seqNodes, n, imax) == max;
+                imaxAndMax
+            
+            else
+                assert forall j: nat :: getStepsTakeByNodeSoFar(seqNodes, n, j) < test by
+                {
+                    forall j: nat 
+                    ensures getStepsTakeByNodeSoFar(seqNodes, n, j) < test
+                    {
+                        assert getStepsTakeByNodeSoFar(seqNodes, n, j) != test;
+                        assert pLemmaGetSeqHonestNodeStates4(seqNodes, n, j, test);
+                        assert getStepsTakeByNodeSoFar(seqNodes, n, j) <= test;
+                    }
+                    // 
+                }
+                // assert forall j: nat :: getStepsTakeByNodeSoFar(seqNodes, n, j) < test;
+                getMaxWhenGetStepsTakeByNodeSoFarIsLimitedHelper(seqNodes, n, test - 1)
+            
+    
+    }
+
+    function getMaxWhenGetStepsTakeByNodeSoFarIsLimited
+    (
+        seqNodes: iseq<Address>,
+        n: Address        
+    ) : (imaxAndMax: (nat, nat))
+    requires pGetStepsTakeByNodeSoFarIsLimited(seqNodes, n)
+    ensures getStepsTakeByNodeSoFar(seqNodes, n, imaxAndMax.0) == imaxAndMax.1;
+    ensures pLemmaGetSeqHonestNodeStates42(seqNodes, n, imaxAndMax.1)
+    {
+        var upperBound: nat :| pLemmaGetSeqHonestNodeStates42(seqNodes, n, upperBound);
+        getMaxWhenGetStepsTakeByNodeSoFarIsLimitedHelper(seqNodes, n, upperBound)
+    }    
+
+    lemma lemmaGetStepsTakeByNodeSoFarIsLimitedHelper
+    (
+        seqNodes: iseq<Address>,
+        n: Address,
+        test: nat
+    ) returns (imax: nat, max: nat)
+    requires  pLemmaGetSeqHonestNodeStates42(seqNodes, n, test)
+    ensures getStepsTakeByNodeSoFar(seqNodes, n, imax) == max;
+    ensures pLemmaGetSeqHonestNodeStates42(seqNodes, n, max)
+    {
+        if test == 0
+        {
+            max := 0;
+            imax := 0;
+            assert getStepsTakeByNodeSoFar(seqNodes, n, imax) == max;
+        }
+        else
+        {
+            if exists j: nat :: getStepsTakeByNodeSoFar(seqNodes, n, j) == test
+            {
+                max := test;
+                imax :| getStepsTakeByNodeSoFar(seqNodes, n, imax) == max;
+                assert getStepsTakeByNodeSoFar(seqNodes, n, imax) == max;
+            }
+            else
+            {
+                forall j: nat 
+                ensures getStepsTakeByNodeSoFar(seqNodes, n, j) < test
+                {
+                    assert getStepsTakeByNodeSoFar(seqNodes, n, j) != test;
+                    assert pLemmaGetSeqHonestNodeStates4(seqNodes, n, j, test);
+                    assert getStepsTakeByNodeSoFar(seqNodes, n, j) <= test;
+                }
+                // assert forall j: nat :: !(getStepsTakeByNodeSoFar(seqNodes, n, j) == test);
+                // assert forall j: nat :: getStepsTakeByNodeSoFar(seqNodes, n, j) < test;
+                imax, max := lemmaGetStepsTakeByNodeSoFarIsLimitedHelper(seqNodes, n, test - 1);
+            }
+        }
+    }
+
+
+    lemma lemmaGetStepsTakeByNodeSoFarIsLimited
+    (
+        seqNodes: iseq<Address>,
+        n: Address        
+    ) returns (imax: nat, max: nat)
+    requires pGetStepsTakeByNodeSoFarIsLimited(seqNodes, n)
+    ensures getStepsTakeByNodeSoFar(seqNodes, n, imax) == max;
+    ensures pLemmaGetSeqHonestNodeStates42(seqNodes, n, max)
+    {
+        var upperBound: nat :| pLemmaGetSeqHonestNodeStates42(seqNodes, n, upperBound);
+        imax, max := lemmaGetStepsTakeByNodeSoFarIsLimitedHelper(seqNodes, n, upperBound);
+    }
+
+    // lemma lemmaGetSeqHonestNodeStates4Recursive(
+    //     dsBehaviour: DSBehaviour,
+    //     configuration: Configuration,       
+    //     n: Address,
+    //     seqNodes: iseq<Address>,
+    //     seqNodeStates: iseq<NodeState>,
+    //     i: nat
+    // )
+    // requires n in dsBehaviour.nodesBehaviours
+    // requires dsBehaviour.nodesBehaviours[n] in QbftSpecificationBuilder(configuration, n).behaviours
+    // requires  |validators([configuration.genesisBlock])| > 0    
+    // requires seqNodeStates == getSeqHonestNodeStates(dsBehaviour, configuration, n, seqNodes)
+    // // ensures var QbftNodeBehaviour := dsBehaviour.nodesBehaviours[n];
+    // //         var stpesTakenByTheNodeSoFar := getStepsTakeByNodeSoFar(seqNodes, n, i);
+    // //         if stpesTakenByTheNodeSoFar == 0 then
+    // //             seqNodeStates[i].blockchain ==  QbftNodeBehaviour.initialBlockchain
+    // //         else
+    // //             var stpesTakenByTheNodeSoFarPrev := stpesTakenByTheNodeSoFar - 1;
+    // //             var step := QbftNodeBehaviour.steps[stpesTakenByTheNodeSoFarPrev];
+    // //             seqNodeStates[i].blockchain == step.newBlockchain  
+
+    predicate pLemmaGetSeqHonestNodeStates4ForAll(
+        dsBehaviour: DSBehaviour,
+        n: Address,
+        seqNodes: iseq<Address>,
+        seqNodeStates: iseq<NodeState>,
+        i: nat
+    )
+    {
+        && n in dsBehaviour.nodesBehaviours
+        && getStepsTakeByNodeSoFarReverse.requires(seqNodes, n, i + 1)
+        && var QbftNodeBehaviour := dsBehaviour.nodesBehaviours[n];
+        QbftNodeBehaviour.steps[i].newBlockchain == seqNodeStates[getStepsTakeByNodeSoFarReverse(seqNodes, n, i + 1)].blockchain        
+    }
+
+    predicate pLemmaGetSeqHonestNodeStates4ForAll2(
+        dsBehaviour: DSBehaviour,
+        n: Address,
+        seqNodes: iseq<Address>,
+        seqDsStates: iseq<DSState>,
+        i: nat
+    )
+    {
+        && getStepsTakeByNodeSoFarReverse.requires(seqNodes, n, i + 1)
+        && n in dsBehaviour.nodesBehaviours
+        && var QbftNodeBehaviour := dsBehaviour.nodesBehaviours[n];
+        var inv := getStepsTakeByNodeSoFarReverse(seqNodes, n, i + 1);
+        && n in seqDsStates[inv].nodes
+        && QbftNodeBehaviour.steps[i].newBlockchain == seqDsStates[inv].nodes[n].blockchain        
+    }    
+
+    lemma lemmaGetSeqHonestNodeStates4ForAll(
+        dsBehaviour: DSBehaviour,
+        configuration: Configuration,       
+        n: Address,
+        seqNodes: iseq<Address>,
+        seqNodeStates: iseq<NodeState>
+    )
+    requires n in dsBehaviour.nodesBehaviours
+    requires IsValidQbftBehaviour(configuration, n, dsBehaviour.nodesBehaviours[n])
+    requires  |validators([configuration.genesisBlock])| > 0    
+    requires seqNodeStates == getSeqHonestNodeStates(dsBehaviour, configuration, n, seqNodes)
+    ensures 
+            if pGetStepsTakeByNodeSoFarIsLimited(seqNodes, n) then
+                forall i: nat | i + 1 <= getMaxWhenGetStepsTakeByNodeSoFarIsLimited(seqNodes, n).1 :: pLemmaGetSeqHonestNodeStates4ForAll(dsBehaviour, n, seqNodes, seqNodeStates, i) 
+            else
+                forall i: nat :: pLemmaGetSeqHonestNodeStates4ForAll(dsBehaviour, n, seqNodes, seqNodeStates, i) 
+    {
+        if !pGetStepsTakeByNodeSoFarIsLimited(seqNodes, n)
+        {
+            forall i: nat 
+            ensures pLemmaGetSeqHonestNodeStates4ForAll(dsBehaviour, n, seqNodes, seqNodeStates, i)          
+            {
+                lemmaGetSeqHonestNodeStates4(dsBehaviour, configuration, n, seqNodes, seqNodeStates, i);
+            }
+        }
+        else
+        {
+            forall i: nat | i + 1 <= getMaxWhenGetStepsTakeByNodeSoFarIsLimited(seqNodes, n).1
+            ensures pLemmaGetSeqHonestNodeStates4ForAll(dsBehaviour, n, seqNodes, seqNodeStates, i)              
+            {
+                lemmaGetSeqHonestNodeStates4(dsBehaviour, configuration, n, seqNodes, seqNodeStates, i);
+            }
+        }
+    }
+
+    lemma lemmaGetSeqHonestNodeStates4(
+        dsBehaviour: DSBehaviour,
+        configuration: Configuration,       
+        n: Address,
+        seqNodes: iseq<Address>,
+        seqNodeStates: iseq<NodeState>,
+        i: nat
+    )
+    requires n in dsBehaviour.nodesBehaviours
+    requires IsValidQbftBehaviour(configuration, n, dsBehaviour.nodesBehaviours[n])
+    requires  |validators([configuration.genesisBlock])| > 0    
+    requires seqNodeStates == getSeqHonestNodeStates(dsBehaviour, configuration, n, seqNodes)
+    requires 
+                || !pGetStepsTakeByNodeSoFarIsLimited(seqNodes, n)
+                || (
+                    && pGetStepsTakeByNodeSoFarIsLimited(seqNodes, n)
+                    && i + 1 <= getMaxWhenGetStepsTakeByNodeSoFarIsLimited(seqNodes, n).1
+                )
+    ensures getStepsTakeByNodeSoFarReverse.requires(seqNodes, n, i + 1);
+    // ensures exists bound: nat :: getStepsTakeByNodeSoFar(seqNodes,n, bound) >= i + 1
+    ensures var QbftNodeBehaviour := dsBehaviour.nodesBehaviours[n];
+            QbftNodeBehaviour.steps[i].newBlockchain == seqNodeStates[getStepsTakeByNodeSoFarReverse(seqNodes, n, i + 1)].blockchain;
+    // ensures var QbftNodeBehaviour := dsBehaviour.nodesBehaviours[n];
+    //         var stpesTakenByTheNodeSoFar := getStepsTakeByNodeSoFar(seqNodes, n, i);
+    //         if stpesTakenByTheNodeSoFar == 0 then
+    //             seqNodeStates[i].blockchain ==  QbftNodeBehaviour.initialBlockchain
+    //         else
+    //             var stpesTakenByTheNodeSoFarPrev := stpesTakenByTheNodeSoFar - 1;
+    //             var step := QbftNodeBehaviour.steps[stpesTakenByTheNodeSoFarPrev];
+    //             seqNodeStates[i].blockchain == step.newBlockchain  
+    // decreases i
+    {
+        var QbftNodeBehaviour := dsBehaviour.nodesBehaviours[n];
+        var nt: iseq<NodeState> :|
+            && NodeInit(nt[0], configuration, n)
+            && QbftNodeBehaviour.initialBlockchain == nt[0].blockchain
+            && (forall i:nat ::
+                    IsValidQbftBehaviourStep(QbftNodeBehaviour, nt ,i)
+                    // var step := QbftNodeBehaviour.steps[i];
+                    // && validNodeState(nt[i])
+                    // && NodeNext(nt[i], step.messageReceived, nt[i+1], step.messagesToSend)
+                    // && step.newBlockchain == nt[i+1].blockchain
+            )
+            &&  seqNodeStates == 
+                imap i: nat :: 
+                    var stepsTakeByNodeSoFar := getStepsTakeByNodeSoFar(seqNodes, n, i);
+                    nt[stepsTakeByNodeSoFar] ;  
+
+        var step := QbftNodeBehaviour.steps[i];
+
+        assert IsValidQbftBehaviourStep(QbftNodeBehaviour, nt, i);
+
+        assert step.newBlockchain == nt[i+1].blockchain;
+
+
+        if pGetStepsTakeByNodeSoFarIsLimited(seqNodes, n)
+        {
+            var (imax, max) := getMaxWhenGetStepsTakeByNodeSoFarIsLimited(seqNodes, n);
+
+            assert i + 1 <= max;
+            // {
+            var inv := getStepsTakeByNodeSoFarReverse(seqNodes, n, i + 1);
+            assert step.newBlockchain == seqNodeStates[getStepsTakeByNodeSoFarReverse(seqNodes, n, i + 1)].blockchain;
+
+            assert exists bound: nat :: getStepsTakeByNodeSoFar(seqNodes,n, bound) >= i + 1;
+            // }
+            // var max :| 
+            //     && (exists j :: getStepsTakeByNodeSoFar(seqNodes, n, j) == max)
+            //     && pLemmaGetSeqHonestNodeStates42(seqNodes, n, max)
+            //     ;
+            // var max :| pLemmaGetSeqHonestNodeStates42(seqNodes, n, max);
+            // if i + 1 <= max 
+            // {
+
+            //     // assert getStepsTakeByNodeSoFar(seqNodes,n, max) >= i + 1;
+            //     // var inv := getStepsTakeByNodeSoFarReverse(seqNodes, n, i + 1);
+            // }
+
+        }
+        else
+        {
+            // assert exists bound :: getStepsTakeByNodeSoFar(seqNodes, n, bound) >= i + 1;
+
+            // assert forall max: nat:: !(forall j: nat :: getStepsTakeByNodeSoFar(seqNodes, n, j) <= max);
+
+            assert !(exists max:nat :: pLemmaGetSeqHonestNodeStates42(seqNodes, n, max));
+            assert forall max: nat :: !pLemmaGetSeqHonestNodeStates42(seqNodes, n, max);
+
+            assert !pLemmaGetSeqHonestNodeStates42(seqNodes, n, i+1);
+            assert exists j:nat :: !pLemmaGetSeqHonestNodeStates4(seqNodes, n, j, i +1);
+            var bound :| !pLemmaGetSeqHonestNodeStates4(seqNodes, n, bound, i +1);
+            assert getStepsTakeByNodeSoFar(seqNodes, n, bound) >= i + 1;
+
+            var inv := getStepsTakeByNodeSoFarReverse(seqNodes, n, i + 1);
+
+            assert step.newBlockchain == seqNodeStates[getStepsTakeByNodeSoFarReverse(seqNodes, n, i + 1)].blockchain;
+
+            assert exists bound: nat :: getStepsTakeByNodeSoFar(seqNodes,n, bound) >= i + 1;
+
+            // assert !(forall max: nat, j:nat :: getStepsTakeByNodeSoFar(seqNodes, n, j) <= max);
+        }
+
+        assert getStepsTakeByNodeSoFarReverse.requires(seqNodes, n, i + 1);
+        
+    }   
+
+    lemma lemmaGetSeqHonestNodeStates5(
+        dsBehaviour: DSBehaviour,
+        configuration: Configuration,       
+        n: Address,
+        seqNodes: iseq<Address>,
+        seqNodeStates: iseq<NodeState>
+    )
+    requires n in dsBehaviour.nodesBehaviours
+    requires IsValidQbftBehaviour(configuration, n, dsBehaviour.nodesBehaviours[n])
+    requires  |validators([configuration.genesisBlock])| > 0    
+    requires seqNodeStates == getSeqHonestNodeStates(dsBehaviour, configuration, n, seqNodes)  
+    ensures seqNodeStates[0].blockchain == dsBehaviour.nodesBehaviours[n].initialBlockchain;
+    {
+        var QbftNodeBehaviour := dsBehaviour.nodesBehaviours[n];
+        var nt: iseq<NodeState> :|
+            && NodeInit(nt[0], configuration, n)
+            && QbftNodeBehaviour.initialBlockchain == nt[0].blockchain
+            && (forall i:nat ::
+                    IsValidQbftBehaviourStep(QbftNodeBehaviour, nt ,i)
+                    // var step := QbftNodeBehaviour.steps[i];
+                    // && validNodeState(nt[i])
+                    // && NodeNext(nt[i], step.messageReceived, nt[i+1], step.messagesToSend)
+                    // && step.newBlockchain == nt[i+1].blockchain
+            )
+            &&  seqNodeStates == 
+                imap i: nat :: 
+                    var stepsTakeByNodeSoFar := getStepsTakeByNodeSoFar(seqNodes, n, i);
+                    nt[stepsTakeByNodeSoFar] ;  
+
+        assert seqNodeStates[0] == nt[0];
+        assert seqNodeStates[0].blockchain == dsBehaviour.nodesBehaviours[n].initialBlockchain;
+    }  
+
+    predicate pLemmaGetSeqHonestNodeStates3ForAll2
+    (
+        dsBehaviour: DSBehaviour,   
+        n: Address,
+        seqNodes: iseq<Address>,
+        seqNodeState: NodeState,
+        i: nat
+    )
+    {
+        && n in dsBehaviour.nodesBehaviours
+        &&
+        var QbftNodeBehaviour := dsBehaviour.nodesBehaviours[n];
+        var stpesTakenByTheNodeSoFar := getStepsTakeByNodeSoFar(seqNodes, n, i);
+        seqNodeState.blockchain ==
+            if stpesTakenByTheNodeSoFar == 0 then
+                QbftNodeBehaviour.initialBlockchain
+            else
+                var stpesTakenByTheNodeSoFarPrev := stpesTakenByTheNodeSoFar - 1;
+                var step := QbftNodeBehaviour.steps[stpesTakenByTheNodeSoFarPrev];
+                step.newBlockchain
+    }  
+
+    predicate pLemmaGetSeqHonestNodeStates3ForAll
+    (
+        dsBehaviour: DSBehaviour,   
+        n: Address,
+        seqNodes: iseq<Address>,
+        seqNodeStates: iseq<NodeState>,
+        i: nat
+    )
+    {
+        && n in dsBehaviour.nodesBehaviours
+        &&
+        var QbftNodeBehaviour := dsBehaviour.nodesBehaviours[n];
+        var stpesTakenByTheNodeSoFar := getStepsTakeByNodeSoFar(seqNodes, n, i);
+        seqNodeStates[i].blockchain ==
+            if stpesTakenByTheNodeSoFar == 0 then
+                QbftNodeBehaviour.initialBlockchain
+            else
+                var stpesTakenByTheNodeSoFarPrev := stpesTakenByTheNodeSoFar - 1;
+                var step := QbftNodeBehaviour.steps[stpesTakenByTheNodeSoFarPrev];
+                step.newBlockchain
+    }
+
+    lemma lemmaGetSeqHonestNodeStates3ForAll(
+        dsBehaviour: DSBehaviour,
+        configuration: Configuration,       
+        n: Address,
+        seqNodes: iseq<Address>,
+        seqNodeStates: iseq<NodeState>
+    )
+    requires n in dsBehaviour.nodesBehaviours
+    requires IsValidQbftBehaviour(configuration, n, dsBehaviour.nodesBehaviours[n])
+    requires  |validators([configuration.genesisBlock])| > 0    
+    requires seqNodeStates == getSeqHonestNodeStates(dsBehaviour, configuration, n, seqNodes)
+
+    ensures 
+            forall i: nat :: pLemmaGetSeqHonestNodeStates3ForAll(dsBehaviour, n, seqNodes, seqNodeStates, i)
+  
+    // decreases i
+    {
+        var QbftNodeBehaviour := dsBehaviour.nodesBehaviours[n];
+        var nt: iseq<NodeState> :|
+            && NodeInit(nt[0], configuration, n)
+            && QbftNodeBehaviour.initialBlockchain == nt[0].blockchain
+            && (forall i:nat ::
+                    IsValidQbftBehaviourStep(QbftNodeBehaviour, nt ,i)
+                    // var step := QbftNodeBehaviour.steps[i];
+                    // && validNodeState(nt[i])
+                    // && NodeNext(nt[i], step.messageReceived, nt[i+1], step.messagesToSend)
+                    // && step.newBlockchain == nt[i+1].blockchain
+            )
+            &&  seqNodeStates == 
+                imap i: nat :: 
+                    var stepsTakeByNodeSoFar := getStepsTakeByNodeSoFar(seqNodes, n, i);
+                    nt[stepsTakeByNodeSoFar] ; 
+
+        forall i: nat 
+        ensures pLemmaGetSeqHonestNodeStates3ForAll(dsBehaviour, n, seqNodes, seqNodeStates, i)
+        
+        // var QbftNodeBehaviour := dsBehaviour.nodesBehaviours[n];
+        //         var stpesTakenByTheNodeSoFar := getStepsTakeByNodeSoFar(seqNodes, n, i);
+        //         if stpesTakenByTheNodeSoFar == 0 then
+        //             seqNodeStates[i].blockchain ==  QbftNodeBehaviour.initialBlockchain
+        //         else
+        //             var stpesTakenByTheNodeSoFarPrev := stpesTakenByTheNodeSoFar - 1;
+        //             var step := QbftNodeBehaviour.steps[stpesTakenByTheNodeSoFarPrev];
+        //             seqNodeStates[i].blockchain == step.newBlockchain          
+        {
+            lemmaGetSeqHonestNodeStates3(
+                dsBehaviour,
+                configuration,
+                n,
+                seqNodes,
+                seqNodeStates,
+                i
+            );
+        }        
+
+    }
+
+    lemma lemmaGetSeqHonestNodeStates(
+        dsBehaviour: DSBehaviour,
+        configuration: Configuration,       
+        n: Address,
+        seqNodes: iseq<Address>,
+        seqNodeStates: iseq<NodeState>
+    )
+    requires n in dsBehaviour.nodesBehaviours
+    requires IsValidQbftBehaviour(configuration, n, dsBehaviour.nodesBehaviours[n])
+    requires  |validators([configuration.genesisBlock])| > 0    
+    requires seqNodeStates == getSeqHonestNodeStates(dsBehaviour, configuration, n, seqNodes)
+    ensures var QbftNodeBehaviour := dsBehaviour.nodesBehaviours[n];
+            forall i:nat ::
+                pGetSeqHonestNodeStatesHelper(QbftNodeBehaviour, seqNodes, seqNodeStates, n, i)
+                // if seqNodes[i] == n then 
+                //     var stepsTakenByNodeSoFar := getStepsTakeByNodeSoFar(seqNodes, n, i);
+                //     var step := QbftNodeBehaviour.steps[stepsTakenByNodeSoFar];
+                //     && validNodeState(seqNodeStates[i])
+                //     && NodeNext(seqNodeStates[i], step.messageReceived, seqNodeStates[i+1], step.messagesToSend)
+                // else
+                //     seqNodeStates[i] == seqNodeStates[i+1]
+    {
+        var QbftNodeBehaviour := dsBehaviour.nodesBehaviours[n];
+        var nt: iseq<NodeState> :|
+            && NodeInit(nt[0], configuration, n)
+            && QbftNodeBehaviour.initialBlockchain == nt[0].blockchain
+            && (forall i:nat ::
+                    IsValidQbftBehaviourStep(QbftNodeBehaviour, nt ,i)
+                    // var step := QbftNodeBehaviour.steps[i];
+                    // && validNodeState(nt[i])
+                    // && NodeNext(nt[i], step.messageReceived, nt[i+1], step.messagesToSend)
+                    // && step.newBlockchain == nt[i+1].blockchain
+            )
+            &&  seqNodeStates == 
+                imap i: nat :: 
+                    var stepsTakeByNodeSoFar := getStepsTakeByNodeSoFar(seqNodes, n, i);
+                    nt[stepsTakeByNodeSoFar] ;   
+
+        // assert forall i: nat :: IsValidQbftBehaviourStep(QbftNodeBehaviour, nt ,i); 
+        // assert forall i: nat :: validNodeState(nt[i]);  
+
+        // forall i: nat 
+        // ensures validNodeState(nt[i]); 
+        // {
+        //     assert IsValidQbftBehaviourStep(QbftNodeBehaviour, nt ,i);
+        //     assert validNodeState(nt[i]); 
+        // }
+
+        forall i: nat 
+        ensures 
+            pGetSeqHonestNodeStatesHelper(QbftNodeBehaviour, seqNodes, seqNodeStates, n, i)
+            // if seqNodes[i] == n then 
+            //     var stepsTakenByNodeSoFar := getStepsTakeByNodeSoFar(seqNodes, n, i);
+            //     var step := QbftNodeBehaviour.steps[stepsTakenByNodeSoFar];
+            //     && validNodeState(seqNodeStates[i])
+            //     && NodeNext(seqNodeStates[i], step.messageReceived, seqNodeStates[i+1], step.messagesToSend)
+            // else
+            //     seqNodeStates[i] == seqNodeStates[i+1]
+        {
+            lemmaGetStepsTakeByNodeSoFar(seqNodes, n, i);
+            if seqNodes[i] == n 
+            {
+                var stepsTakenByNodeSoFar := getStepsTakeByNodeSoFar(seqNodes, n, i);
+                assert getStepsTakeByNodeSoFar(seqNodes, n, i + 1) == stepsTakenByNodeSoFar + 1;
+
+                assert seqNodeStates[i] == nt[stepsTakenByNodeSoFar];
+
+                lemmaGetSeqHonestNodeStatesHelper(QbftNodeBehaviour, nt, stepsTakenByNodeSoFar);
+
+                // assert IsValidQbftBehaviourStep(QbftNodeBehaviour, nt ,stepsTakenByNodeSoFar);
+                assert validNodeState(seqNodeStates[i]); 
+                assert validNodeState(nt[stepsTakenByNodeSoFar]); 
+                var step := QbftNodeBehaviour.steps[stepsTakenByNodeSoFar];
+                assert NodeNext(nt[stepsTakenByNodeSoFar], step.messagesReceived, nt[stepsTakenByNodeSoFar+1], step.messagesToSend);
+                assert NodeNext(seqNodeStates[i], step.messagesReceived, seqNodeStates[i+1], step.messagesToSend);
+
+               
+            }
+            else
+            {
+                assert seqNodeStates[i] == seqNodeStates[i+1];
+            }
+
+
+        }
+
+
+        // forall i: nat 
+        // {
+        //         assert seqNodeStates[i].blockchain == nt[getStepsTakeByNodeSoFar(seqNodes, n, i)].blockchain;     
+
+        //         assert seqNodeStates[i+1].blockchain == QbftNodeBehaviour.steps[getStepsTakeByNodeSoFar(seqNodes, n, i)].newBlockchain;             
+        // }
+    }
+
+    // function getSeqAdvStates(
+    //     dsBehaviour: DSBehaviour,
+    //     configuration: Configuration,       
+    //     n: Address,
+    //     seqNodes: iseq<Address>
+    // ): (ret: iseq<Adversary>)
+    // requires n in dsBehaviour.nodesBehaviours
+    // requires dsBehaviour.adversaryBehaviour in AdversarySpecificationBuilder(configuration, n).behaviours
+    // requires  |validators([configuration.genesisBlock])| > 0
+    // // ensures NodeInit(ret[0], configuration, n)
+    // {
+    //     var QbftNodeBehaviour := dsBehaviour.nodesBehaviours[n];
+    //     var seqAdvStates: iseq<Adversary> :|
+    //         && AdversaryInit(seqAdvStates[0], configuration)
+    //         && seqAdvStates[0].byz == allNodes - dsBehaviour.nodesBehaviours.Keys
+    //         && (forall i:nat ::
+    //                 var step := dsBehaviour.adversaryBehaviour.steps[i];
+    //                 && AdversaryNext(seqAdvStates[i], step.messageReceived, seqAdvStates[i+1], step.messagesToSend)
+    //         );
+    //     imap i: nat :: 
+    //         var stepsTakeByNodeSoFar := getStepsTakeByNodeSoFar(seqNodes, n, i);
+    //         nt[stepsTakeByNodeSoFar]   
+    // }  
+
+
+    function getSeqHonestNodeStates(
+        dsBehaviour: DSBehaviour,
+        configuration: Configuration,       
+        n: Address,
+        seqNodes: iseq<Address>
+    ): (ret: iseq<NodeState>)
+    requires n in dsBehaviour.nodesBehaviours
+    requires IsValidQbftBehaviour(configuration, n, dsBehaviour.nodesBehaviours[n])
+    requires  |validators([configuration.genesisBlock])| > 0
+    // ensures NodeInit(ret[0], configuration, n)
+    {
+        var QbftNodeBehaviour := dsBehaviour.nodesBehaviours[n];
+        var nt: iseq<NodeState> :|
+            && NodeInit(nt[0], configuration, n)
+            && QbftNodeBehaviour.initialBlockchain == nt[0].blockchain
+            && (forall i:nat ::
+                    IsValidQbftBehaviourStep(QbftNodeBehaviour, nt ,i)
+                    // var step := QbftNodeBehaviour.steps[i];
+                    // && validNodeState(nt[i])
+                    // && NodeNext(nt[i], step.messageReceived, nt[i+1], step.messagesToSend)
+                    // && step.newBlockchain == nt[i+1].blockchain
+            );
+        imap i: nat :: 
+            var stepsTakeByNodeSoFar := getStepsTakeByNodeSoFar(seqNodes, n, i);
+            nt[stepsTakeByNodeSoFar]   
+    }    
+
+    function getSeqNodeStates(
+        dsBehaviour: DSBehaviour,
+        configuration: Configuration,       
+        n: Address,
+        honestNodes: set<Address>,
+        seqNodes: iseq<Address>
+    ): (seqNodeStates: iseq<NodeState>)
+    requires n in honestNodes ==> n in dsBehaviour.nodesBehaviours
+    requires n in honestNodes ==> IsValidQbftBehaviour(configuration, n, dsBehaviour.nodesBehaviours[n])
+    requires  |validators([configuration.genesisBlock])| > 0
+    // ensures 
+    // ensures
+    //     var QbftNodeBehaviour := dsBehaviour.nodesBehaviours[n]; 
+    //     n in honestNodes ==>
+    //         (
+    //             forall i:nat ::
+    //                 if seqNodes[i] == n then 
+    //                     var stepsTakenByNodeSoFar := getStepsTakeByNodeSoFar(seqNodes, n, i);
+    //                     var step := QbftNodeBehaviour.steps[stepsTakenByNodeSoFar];
+    //                     && validNodeState(seqNodeStates[i])
+    //                     && NodeNext(seqNodeStates[i], step.messageReceived, seqNodeStates[i+1], step.messagesToSend)
+    //                 else
+    //                     seqNodeStates[i] == seqNodeStates[i+1]
+    //         )
+    // ensures NodeInit(ret[0], configuration, n)
+    {
+        if n in honestNodes then
+                var ret := getSeqHonestNodeStates(dsBehaviour, configuration, n, seqNodes);
+                ret
+            else
+                getDummySeqNodes(configuration, n)    
+    }    
+
+    lemma lemmajkfladjklfaGetSeqNodeStates(
+       dsBehaviour: DSBehaviour,
+       configuration: Configuration,
+       allNodes: set<Address>,
+       honestNodes: set<Address>,
+       seqNodes: iseq<Address>     
+    ) returns ( seqsNodeStates: map<Address, iseq<NodeState>>)
+    requires IsValidConfiguration(configuration)
+    requires dsBehaviour in DSSpecificationBuilder(configuration).behaviours
+    requires  |validators([configuration.genesisBlock])| > 0
+    requires allNodes == seqToSet(configuration.nodes);
+    requires honestNodes == dsBehaviour.nodesBehaviours.Keys; 
+    ensures  seqsNodeStates.Keys == allNodes  
+    ensures 
+            forall n | n in allNodes ::
+                if n in honestNodes then
+                    (
+                        var QbftNodeBehaviour := dsBehaviour.nodesBehaviours[n]; 
+                        var seqNodeStates := seqsNodeStates[n];
+                        forall i:nat ::
+                            pGetSeqHonestNodeStatesHelper(QbftNodeBehaviour, seqNodes, seqNodeStates, n, i)
+                    )   
+                else
+                    (forall i: nat :: seqsNodeStates[n][0] == seqsNodeStates[n][i])
+    ensures forall n | n in allNodes :: NodeInit(seqsNodeStates[n][0], configuration, n)
+    ensures forall n, i:nat | n in honestNodes :: validNodeState(seqsNodeStates[n][i])
+    ensures forall n, i:nat | n in honestNodes :: pLemmaGetSeqHonestNodeStates3ForAll(dsBehaviour, n, seqNodes, seqsNodeStates[n], i)
+    ensures forall n | n in honestNodes ::
+            if pGetStepsTakeByNodeSoFarIsLimited(seqNodes, n) then
+                forall i: nat | i + 1 <= getMaxWhenGetStepsTakeByNodeSoFarIsLimited(seqNodes, n).1 :: pLemmaGetSeqHonestNodeStates4ForAll(dsBehaviour, n, seqNodes, seqsNodeStates[n], i) 
+            else
+                forall i: nat :: pLemmaGetSeqHonestNodeStates4ForAll(dsBehaviour, n, seqNodes, seqsNodeStates[n], i) 
+    ensures forall n | n in honestNodes  ::
+        (seqsNodeStates[n][0].blockchain == dsBehaviour.nodesBehaviours[n].initialBlockchain)       
+    {
+        seqsNodeStates
+        
+        :=
+            map n | n in allNodes ::
+                getSeqNodeStates(dsBehaviour, configuration, n, honestNodes, seqNodes)
+            ;    
+
+        forall n | n in allNodes
+        ensures
+            if n in honestNodes then
+                (
+                    var QbftNodeBehaviour := dsBehaviour.nodesBehaviours[n]; 
+                    var seqNodeStates := seqsNodeStates[n];
+                    forall i:nat ::
+                        pGetSeqHonestNodeStatesHelper(QbftNodeBehaviour, seqNodes, seqNodeStates, n, i)
+                )  
+            else
+                (
+                    forall i: nat :: seqsNodeStates[n][0] == seqsNodeStates[n][i]
+                )      
+        ensures NodeInit(seqsNodeStates[n][0], configuration, n);
+        ensures n in honestNodes ==> (forall i:nat :: validNodeState(seqsNodeStates[n][i]))
+        ensures n in honestNodes ==> (forall i: nat :: pLemmaGetSeqHonestNodeStates3ForAll(dsBehaviour, n, seqNodes, seqsNodeStates[n], i))
+        ensures n in honestNodes ==>
+            if pGetStepsTakeByNodeSoFarIsLimited(seqNodes, n) then
+                forall i: nat | i + 1 <= getMaxWhenGetStepsTakeByNodeSoFarIsLimited(seqNodes, n).1 :: pLemmaGetSeqHonestNodeStates4ForAll(dsBehaviour, n, seqNodes, seqsNodeStates[n], i) 
+            else
+                forall i: nat :: pLemmaGetSeqHonestNodeStates4ForAll(dsBehaviour, n, seqNodes, seqsNodeStates[n], i)  
+        ensures n in honestNodes ==>  (seqsNodeStates[n][0].blockchain == dsBehaviour.nodesBehaviours[n].initialBlockchain)  
+        {
+            var seqNodeStates := seqsNodeStates[n];
+
+            if n in honestNodes
+            {
+                assert seqNodeStates == getSeqHonestNodeStates(dsBehaviour, configuration, n, seqNodes);
+                lemmaGetSeqHonestNodeStates(dsBehaviour, configuration, n, seqNodes, seqNodeStates);
+                assert NodeInit(seqNodeStates[0], configuration, n);
+
+                forall i:nat 
+                ensures validNodeState(seqNodeStates[i])
+                {
+                    lemmaGetSeqHonestNodeStates2(dsBehaviour, configuration, n, seqNodes, seqNodeStates, i);
+                }
+
+                lemmaGetSeqHonestNodeStates3ForAll(dsBehaviour, configuration, n, seqNodes, seqsNodeStates[n]);
+                lemmaGetSeqHonestNodeStates4ForAll(dsBehaviour, configuration, n, seqNodes, seqsNodeStates[n]);
+
+                lemmaGetSeqHonestNodeStates5(dsBehaviour, configuration, n, seqNodes, seqsNodeStates[n]);
+            }
+            else
+            {
+                assert NodeInit(seqNodeStates[0], configuration, n);
+                assert forall i: nat :: seqNodeStates[0] == seqNodeStates[i];
+            }
+        } 
+
+         
+ 
+    }
+
+    lemma lemmajkfladjklfaGetDsStates(
+       configuration: Configuration,
+       seqEnvStates: iseq<Network>,
+       seqNodeStates: map<Address, iseq<NodeState>>,
+       seqAdvStates: iseq<Adversary>,
+       allNodes: set<Address>
+    ) returns (dsStates: iseq<DSState>)
+    requires seqNodeStates.Keys == allNodes
+    ensures dsStates ==             
+            imap i: nat ::
+                DSState(
+                    configuration,
+                    seqEnvStates[i],
+                    map n | n in allNodes :: seqNodeStates[n][i],
+                    seqAdvStates[i]
+                );
+    ensures forall i: nat :: dsStates[i].nodes.Keys == allNodes
+    {
+        dsStates := 
+            imap i: nat ::
+                DSState(
+                    configuration,
+                    seqEnvStates[i],
+                    map n | n in allNodes :: seqNodeStates[n][i],
+                    seqAdvStates[i]
+                );
+
+    }
+
+    lemma lemmajkfladjklfaGetDsStatesHelper(
+        dsBehaviour: DSBehaviour,
+        configuration: Configuration,
+        seqAdvStates: iseq<Adversary>,
+        i: nat
+    )
+    // requires seqNodeStates.Keys == allNodes
+    // requires  dsStates == 
+    //             imap i: nat ::
+    //                 DSState(
+    //                     configuration,
+    //                     seqEnvStates[i],
+    //                     map n | n in allNodes :: seqNodeStates[n][i],
+    //                     seqAdvStates[i]
+    //                 );
+    // requires dsBehaviour.adversaryBehaviour in AdversarySpecificationBuilder(configuration).behaviours
+    requires    && AdversaryInit(seqAdvStates[0], configuration)
+                && (forall i:nat ::
+                        pLemmajkfladjklfaGetAdvStatesHelper(dsBehaviour, seqAdvStates, i)
+                        // var step := dsBehaviour.adversaryBehaviour.steps[i];
+                        // && AdversaryNext(seqAdvStates[i], step.messageReceived, seqAdvStates[i+1], step.messagesToSend)
+                )
+    ensures seqAdvStates[0].byz == seqAdvStates[i].byz
+    {
+        // assert seqAdvStates[0].byz == seqAdvStates[0].byz;
+        for j := 0 to i
+            invariant seqAdvStates[0].byz == seqAdvStates[j].byz
+        {
+            var step := dsBehaviour.adversaryBehaviour.steps[j];
+            assert pLemmajkfladjklfaGetAdvStatesHelper(dsBehaviour, seqAdvStates, j);
+            assert AdversaryNext(seqAdvStates[j], step.messageReceived, seqAdvStates[j+1], step.messagesToSend);
+            assert seqAdvStates[j].byz == seqAdvStates[j+1].byz;
+        }
+    } 
+
+    lemma lemmajkfladjklfaHelper2(
+        s: NodeState,
+        mIn: set<QbftMessage>,
+        s': NodeState,
+        mOut: set<QbftMessageWithRecipient>,
+        mIn': set<QbftMessage>,
+        mOut': set<QbftMessageWithRecipient>
+    )
+    requires validNodeState(s)
+    requires NodeNext(s, mIn, s', mOut)
+    requires mIn == mIn' 
+    requires mOut == mOut' 
+    ensures NodeNext(s, mIn', s', mOut')
+    {
+
+    }
+
+    lemma lemmajkfladjklfaHelper3(
+        s: DSState,
+        s': DSState,
+        allNodes: set<Address>,
+        node: Address
+    )   
+    requires s.nodes.Keys == s'.nodes.Keys == allNodes;   
+    requires node in allNodes
+    requires forall node' | node' in allNodes && node != node' :: s.nodes[node'] == s'.nodes[node'];
+    ensures s'.nodes == s.nodes[node := s'.nodes[node]];
+    {
+
+    }   
+
+    lemma lemmajkfladjklfaHelper4(
+        s: DSState,
+        s': DSState,
+        allNodes: set<Address>
+    )   
+    requires s.nodes.Keys == s'.nodes.Keys == allNodes;   
+    requires forall node' | node' in allNodes :: s.nodes[node'] == s'.nodes[node'];
+    ensures s'.nodes == s.nodes;
+    {
+
+    }      
+
+
+    lemma lemmajkfladjklfaHelper5(
+        s: Adversary,
+        mIn: set<QbftMessage>,
+        s': Adversary,
+        mOut: set<QbftMessageWithRecipient>,
+        mIn': set<QbftMessage>,
+        mOut': set<QbftMessageWithRecipient>
+    )
+    requires AdversaryNext(s, mIn, s', mOut)
+    requires mIn == mIn' 
+    requires mOut == mOut' 
+    ensures AdversaryNext(s, mIn', s', mOut')
+    {
+
+    }     
+
+    // lemma lemmajkfladjklfaHelper6(
+    //    dsBehaviour: DSBehaviour,
+    //    configuration: Configuration,
+    //    dsStates: iseq<DSState>,
+    //    i: nat
+    // )     
+    // requires IsValidConfiguration(configuration)
+    // requires dsBehaviour in DSSpecificationBuilder(configuration).behaviours
+    // requires  |validators([configuration.genesisBlock])| > 0
+    // // ensures forall i: nat :: validDSState(dsStates[i]);    
+    // {
+    //         var s := dsStates[i];
+    //         var s' := dsStates[i+1];
+    //         var environmentStep := dsBehaviour.environmentBehaviour.steps[i];
+    //         var messagesReceivedWithoutRecipient := (set mr:QbftMessageWithRecipient | mr in environmentStep.messagesReceivedByTheNodes :: mr.message);            
+
+
+    //         assert s'.configuration == s.configuration;
+    //         assert s.environment == seqEnvStates[i];
+    //         assert s'.environment == seqEnvStates[i+1];
+    //         assert lemmajkfladjklfaGetEnvStatesHelper(seqEnvStates, dsBehaviour.environmentBehaviour, i);
+    //         assert NetworkNext(s.environment,s'.environment,environmentStep.messagesSentByTheNodes,environmentStep.messagesReceivedByTheNodes);  
+    //         var node := seqNodes[i];
+    //         assert DSSpecificationBuilderHelper(dsBehaviour, allNodes, honestNodes, seqNodes, i);
+    //         assert s.nodes.Keys == allNodes;
+    //         assert node in s.nodes;   
+    //         assert s.nodes.Keys == s'.nodes.Keys; 
+    //         assert s.configuration == configuration;  
+            
+    //         // lemmajkfladjklfaGetDsStatesHelper(dsBehaviour, dsStates, configuration, seqAdvStates, i);
+
+    //         if isHonest(s, node)
+    //         {
+    //             assert node in allNodes;
+    //             assert node !in s.adversary.byz;
+    //             assert node !in byzNodes;
+    //             assert node in honestNodes;
+
+    //             var QbftNodeBehaviour := dsBehaviour.nodesBehaviours[node];
+
+    //             assert pGetSeqHonestNodeStatesHelper(QbftNodeBehaviour, seqNodes, seqNodeStates[node], node, i);
+
+    //             var stepsTakenByNodeSoFar := getStepsTakeByNodeSoFar(seqNodes, node, i);
+    //             var step := QbftNodeBehaviour.steps[stepsTakenByNodeSoFar];                
+
+    //             assert
+    //             && validNodeState(seqNodeStates[node][i])
+    //             && NodeNext(seqNodeStates[node][i], step.messageReceived, seqNodeStates[node][i+1], step.messagesToSend)  
+    //             ;    
+
+    //             forall node' | node' in allNodes && node' != node 
+    //             ensures seqNodeStates[node'][i] == seqNodeStates[node'][i+1];
+    //             {
+    //                 // assert 
+    //                 // lemmaGetSeqHonestNodeStates(dsBehaviour, configuration, node', seqNodes, seqNodeStates[node']);
+    //                 // assert seqNodeStates[node'][i] == seqNodeStates[node'][i+1];
+    //                 assert seqNodes[i] != node';
+    //                 if node' in honestNodes 
+    //                 {
+    //                     assert node' in allNodes;
+    //                     assert pGetSeqHonestNodeStatesHelper(dsBehaviour.nodesBehaviours[node'], seqNodes, seqNodeStates[node'], node', i);
+    //                     assert seqNodeStates[node'][i] == seqNodeStates[node'][i+1];
+    //                 }
+    //                 else
+    //                 {
+    //                     assert seqNodeStates[node'][i] == seqNodeStates[node'][i+1];
+    //                 }
+    //             }     
+
+    //             // assert  s'.nodes == s.nodes[node := s'.nodes[node]];
+    //             assert s.nodes == map n | n in allNodes :: seqNodeStates[n][i];
+    //             assert s'.nodes == map n | n in allNodes :: seqNodeStates[n][i+1];
+    //             assert forall node' | node' in allNodes && node != node' :: s.nodes[node'] == s'.nodes[node'];
+    //             assert s.nodes.Keys == s'.nodes.Keys == allNodes;
+    //             lemmajkfladjklfaHelper3(s, s', allNodes, node);
+    //             assert s'.nodes == s.nodes[node := s'.nodes[node]];
+
+    //             lemmaGetStepsTakeByAdversarySoFar(seqNodes, byzNodes, i);
+
+    //             // assert get(seqNodes, byzNodes, i) == lemmaGetStepsTakeByAdversarySoFar(seqNodes, byzNodes, i+1);
+    //             assert s.adversary == s'.adversary;
+
+    //             assert step.messagesToSend == environmentStep.messagesSentByTheNodes;
+    //             assert step.messageReceived == messagesReceivedWithoutRecipient; 
+
+    //             lemmajkfladjklfaHelper2(seqNodeStates[node][i], step.messageReceived, seqNodeStates[node][i+1], step.messagesToSend, messagesReceivedWithoutRecipient, environmentStep.messagesSentByTheNodes);
+
+    //             assert NodeNext(seqNodeStates[node][i], messagesReceivedWithoutRecipient, seqNodeStates[node][i+1], environmentStep.messagesSentByTheNodes);
+                
+
+
+    //         }  
+    //         else
+    //         {
+    //             assert node in byzNodes;
+    //             var stepsTakenByNodeSoFar := getStepsTakeByAversarySoFar(seqNodes, byzNodes, i);
+    //             lemmaGetStepsTakeByAdversarySoFar(seqNodes, byzNodes, i);
+    //             var stepsTakenByNodeSoFarPlusOne := getStepsTakeByAversarySoFar(seqNodes, byzNodes, i + 1);
+    //             assert stepsTakenByNodeSoFar + 1 == stepsTakenByNodeSoFarPlusOne;
+    //             var adversaryBehaviour := dsBehaviour.adversaryBehaviour;
+    //             // var seqAdvStates := adversaryBehaviour.steps;
+    //             var step := adversaryBehaviour.steps[stepsTakenByNodeSoFar];
+
+
+
+    //             assert AdversaryNext(seqAdvStates[i], step.messageReceived, seqAdvStates[i+1], step.messagesToSend);
+
+    //             assert AdversaryNext(s.adversary, step.messageReceived, s'.adversary, step.messagesToSend);
+
+    //             lemmajkfladjklfaHelper5(s.adversary, step.messageReceived, s'.adversary, step.messagesToSend, messagesReceivedWithoutRecipient, environmentStep.messagesSentByTheNodes);
+
+    //             assert AdversaryNext(s.adversary, messagesReceivedWithoutRecipient, s'.adversary, environmentStep.messagesSentByTheNodes);
+
+    //             forall node' | node' in allNodes 
+    //             ensures seqNodeStates[node'][i] == seqNodeStates[node'][i+1];
+    //             {
+    //                 // assert 
+    //                 // lemmaGetSeqHonestNodeStates(dsBehaviour, configuration, node', seqNodes, seqNodeStates[node']);
+    //                 // assert seqNodeStates[node'][i] == seqNodeStates[node'][i+1];
+
+    //                 if node' in honestNodes
+    //                 {
+    //                     assert seqNodes[i] != node';
+
+    //                     assert node' in allNodes;
+    //                     assert pGetSeqHonestNodeStatesHelper(dsBehaviour.nodesBehaviours[node'], seqNodes, seqNodeStates[node'], node', i);
+    //                     assert seqNodeStates[node'][i] == seqNodeStates[node'][i+1];
+    //                 }
+    //                 else
+    //                 {
+    //                     assert seqNodeStates[node'][i] == seqNodeStates[node'][i+1];
+    //                 }
+
+    //             }                 
+
+    //             lemmajkfladjklfaHelper4(s, s', allNodes);
+
+    //             assert s.nodes == s'.nodes;
+
+    //             // assert step.messagesToSend == environmentStep.messagesSentByTheNodes;
+
+    //             // assert AdversaryNext(seqAdvStates[i], step.messageReceived, seqAdvStates[i+1], step.messagesToSend)
+    //         } 
+
+    //         assert forall n | n in honestNodes :: validNodeState(seqNodeStates[n][i]);
+    //         // lemmaGetSeqHonestNodeStates2(dsBehaviour, configuration, )
+
+    //         // forall node': Address | node' in honestNodes
+    //         // {
+    //         //     // var QbftNodeBehaviour := dsBehaviour.nodesBehaviours[node'];
+    //         //     // assert pGetSeqHonestNodeStatesHelper(QbftNodeBehaviour, seqNodes, seqNodeStates[node'], node', i);
+
+    //         //     // assert validNodeState(seqNodeStates[node'][i]);
+    //         //     lemmaGetSeqHonestNodeStates2(dsBehaviour, configuration, node', seqNodes, seqNodeStates[node'], i);
+    //         // }
+
+    //         // assert
+    //         // && NetworkNext(s.environment,s'.environment,environmentStep.messagesSentByTheNodes,environmentStep.messagesReceivedByTheNodes)
+    //         // && (forall mr:QbftMessageWithRecipient | mr in environmentStep.messagesReceivedByTheNodes :: mr.recipient == node)
+    //         // && var messageReceived := set mr:QbftMessageWithRecipient | mr in environmentStep.messagesReceivedByTheNodes :: mr.message;
+    //         // && node in s.nodes
+    //         // && s'.nodes.Keys == s.nodes.Keys
+    //         // && (
+    //         //     if isHonest(s,node) then
+    //         //         && s'.nodes == s.nodes[node := s'.nodes[node]]
+    //         //         && s'.adversary == s.adversary
+    //         //         && NodeNext(s.nodes[node],messageReceived,s'.nodes[node],environmentStep.messagesSentByTheNodes)
+    //         //     else
+    //         //         && s'.nodes == s.nodes
+    //         //         && AdversaryNext(s.adversary,messageReceived,s'.adversary,environmentStep.messagesSentByTheNodes)
+    //         // )
+    //         // && s'.configuration == s.configuration  
+    //         // ;          
+
+    //         assert DSNextNode(s, s', environmentStep.messagesSentByTheNodes, environmentStep.messagesReceivedByTheNodes, node);        
+    // }
+
+    predicate pLemmajkfladjklfa(
+        dsStates: iseq<DSState>,
+        seqNodes: iseq<Address>,
+        environmentBehaviour: EnvironmentSpecificationBehaviour,
+        i: nat
+    )
+    {
+        var environmentStep := environmentBehaviour.steps[i];
+        && validDSState(dsStates[i])
+        && DSNextNode(dsStates[i], dsStates[i+1], environmentStep.messagesSentByTheNodes, environmentStep.messagesReceivedByTheNodes, seqNodes[i])     
+    }
+
+    lemma lemmajkfladjklfa (
+       dsBehaviour: DSBehaviour,
+       configuration: Configuration,
+       seqNodes: iseq<Address>
+    ) returns (dsStates: iseq<DSState>)
+    requires IsValidConfiguration(configuration)
+    requires dsBehaviour in DSSpecificationBuilder(configuration).behaviours
+    requires  |validators([configuration.genesisBlock])| > 0
+    requires    var allNodes := seqToSet(configuration.nodes);
+                pLemmajkfladjklfaGetSeqNodes(dsBehaviour, allNodes, seqNodes)
+
+    // ensures forall i: nat :: validDSState(dsStates[i]);
+    // ensures forall i: nat :: seqNodes[i] in dsStates[i].nodes
+    ensures DSInit(dsStates[0], configuration)
+    ensures 
+            forall i: nat :: pLemmajkfladjklfa(dsStates, seqNodes, dsBehaviour.environmentBehaviour, i)
+    //                 var environmentStep := dsBehaviour.environmentBehaviour.steps[i];
+    //                 && validDSState(dsStates[i])
+    //                 && DSNextNode(dsStates[i], dsStates[i+1], environmentStep.messagesSentByTheNodes, environmentStep.messagesReceivedByTheNodes, seqNodes[i]);    
+
+    ensures forall i: nat :: dsBehaviour.nodesBehaviours.Keys <= dsStates[i].nodes.Keys
+    ensures forall n, i:nat | n in dsBehaviour.nodesBehaviours.Keys :: pLemmaGetSeqHonestNodeStates3ForAll2(dsBehaviour, n, seqNodes, dsStates[i].nodes[n], i);    
+    ensures forall n: Address, i: nat :: (isHonest(dsStates[i], n) <==> n in dsBehaviour.nodesBehaviours.Keys);
+    ensures forall n | n in dsBehaviour.nodesBehaviours.Keys ::
+            if pGetStepsTakeByNodeSoFarIsLimited(seqNodes, n) then
+                forall i: nat | i + 1 <= getMaxWhenGetStepsTakeByNodeSoFarIsLimited(seqNodes, n).1 :: pLemmaGetSeqHonestNodeStates4ForAll2(dsBehaviour, n, seqNodes, dsStates, i) 
+            else
+                forall i: nat :: pLemmaGetSeqHonestNodeStates4ForAll2(dsBehaviour, n, seqNodes, dsStates, i)  
+    ensures forall n | n in dsBehaviour.nodesBehaviours.Keys  ::
+        (dsStates[0].nodes[n].blockchain == dsBehaviour.nodesBehaviours[n].initialBlockchain)                 
+    {
+        var allNodes := seqToSet(configuration.nodes);
+        var honestNodes := dsBehaviour.nodesBehaviours.Keys;
+        var byzNodes := allNodes - honestNodes;
+       
+        // seqNodes := lemmajkfladjklfaGetSeqNodes(dsBehaviour, configuration, allNodes);
+             
+
+        var seqAdvStates := lemmajkfladjklfaGetAdvStates(dsBehaviour, configuration, allNodes, seqNodes);
+
+        var seqEnvStates := lemmajkfladjklfaGetEnvStates(dsBehaviour, configuration);           
+
+        var seqNodeStates := lemmajkfladjklfaGetSeqNodeStates(dsBehaviour, configuration, allNodes, honestNodes, seqNodes);
+
+        dsStates := lemmajkfladjklfaGetDsStates(
+            configuration,
+            seqEnvStates,
+            seqNodeStates,
+            seqAdvStates,
+            allNodes
+        );
+
+        assert forall i: nat :: dsStates[i].adversary == seqAdvStates[i];
+
+        forall i:nat, n: Address //| n in honestNodes
+        ensures isHonest(dsStates[i], n) <==> n in honestNodes
+        {
+            if n in honestNodes
+            {
+                assert n in dsStates[i].nodes;
+                assert n !in seqAdvStates[0].byz;
+                assert n !in seqAdvStates[i].byz;
+                assert isHonest(dsStates[i], n);
+            }
+
+            if isHonest(dsStates[i], n)
+            {
+                assert n in honestNodes;
+            }
+        }    
+
+        // assert forall i: nat, n: Address :: (isHonest(dsStates[i], n) <==> n in honestNodes);
+
+        assert DSInit(dsStates[0], configuration);
+
+        forall i: nat 
+        ensures pLemmajkfladjklfa(dsStates, seqNodes, dsBehaviour.environmentBehaviour, i)
+        // ensures validDSState(dsStates[i]);
+        // ensures 
+        //             var environmentStep := dsBehaviour.environmentBehaviour.steps[i];
+        //             DSNextNode(dsStates[i], dsStates[i+1], environmentStep.messagesSentByTheNodes, environmentStep.messagesReceivedByTheNodes, seqNodes[i]);
+        {
+            var s := dsStates[i];
+            var s' := dsStates[i+1];
+            var environmentStep := dsBehaviour.environmentBehaviour.steps[i];
+            var messagesReceivedWithoutRecipient := (set mr:QbftMessageWithRecipient | mr in environmentStep.messagesReceivedByTheNodes :: mr.message);            
+
+
+            assert s'.configuration == s.configuration;
+            assert s.environment == seqEnvStates[i];
+            assert s'.environment == seqEnvStates[i+1];
+            assert lemmajkfladjklfaGetEnvStatesHelper(seqEnvStates, dsBehaviour.environmentBehaviour, i);
+            assert NetworkNext(s.environment,s'.environment,environmentStep.messagesSentByTheNodes,environmentStep.messagesReceivedByTheNodes);  
+            var node := seqNodes[i];
+            assert DSSpecificationBuilderHelper(dsBehaviour, allNodes, seqNodes, i);
+            assert s.nodes.Keys == allNodes;
+            assert node in s.nodes;   
+            assert s.nodes.Keys == s'.nodes.Keys; 
+            assert s.configuration == configuration;  
+            
+            // lemmajkfladjklfaGetDsStatesHelper(dsBehaviour, dsStates, configuration, seqAdvStates, i);
+
+            if isHonest(s, node)
+            {
+                assert node in allNodes;
+                assert node !in s.adversary.byz;
+                assert node !in byzNodes;
+                assert node in honestNodes;
+
+                var QbftNodeBehaviour := dsBehaviour.nodesBehaviours[node];
+
+                assert pGetSeqHonestNodeStatesHelper(QbftNodeBehaviour, seqNodes, seqNodeStates[node], node, i);
+
+                var stepsTakenByNodeSoFar := getStepsTakeByNodeSoFar(seqNodes, node, i);
+                var step := QbftNodeBehaviour.steps[stepsTakenByNodeSoFar];                
+
+                assert
+                && validNodeState(seqNodeStates[node][i])
+                && NodeNext(seqNodeStates[node][i], step.messagesReceived, seqNodeStates[node][i+1], step.messagesToSend)  
+                ;    
+
+                forall node' | node' in allNodes && node' != node 
+                ensures seqNodeStates[node'][i] == seqNodeStates[node'][i+1];
+                {
+                    // assert 
+                    // lemmaGetSeqHonestNodeStates(dsBehaviour, configuration, node', seqNodes, seqNodeStates[node']);
+                    // assert seqNodeStates[node'][i] == seqNodeStates[node'][i+1];
+                    assert seqNodes[i] != node';
+                    if node' in honestNodes 
+                    {
+                        assert node' in allNodes;
+                        assert pGetSeqHonestNodeStatesHelper(dsBehaviour.nodesBehaviours[node'], seqNodes, seqNodeStates[node'], node', i);
+                        assert seqNodeStates[node'][i] == seqNodeStates[node'][i+1];
+                    }
+                    else
+                    {
+                        assert seqNodeStates[node'][i] == seqNodeStates[node'][i+1];
+                    }
+                }     
+
+                // assert  s'.nodes == s.nodes[node := s'.nodes[node]];
+                assert s.nodes == map n | n in allNodes :: seqNodeStates[n][i];
+                assert s'.nodes == map n | n in allNodes :: seqNodeStates[n][i+1];
+                assert forall node' | node' in allNodes && node != node' :: s.nodes[node'] == s'.nodes[node'];
+                assert s.nodes.Keys == s'.nodes.Keys == allNodes;
+                lemmajkfladjklfaHelper3(s, s', allNodes, node);
+                assert s'.nodes == s.nodes[node := s'.nodes[node]];
+
+                lemmaGetStepsTakeByAdversarySoFar(seqNodes, byzNodes, i);
+
+                // assert get(seqNodes, byzNodes, i) == lemmaGetStepsTakeByAdversarySoFar(seqNodes, byzNodes, i+1);
+                assert s.adversary == s'.adversary;
+
+                assert step.messagesToSend == environmentStep.messagesSentByTheNodes;
+                assert step.messagesReceived == messagesReceivedWithoutRecipient; 
+
+                lemmajkfladjklfaHelper2(seqNodeStates[node][i], step.messagesReceived, seqNodeStates[node][i+1], step.messagesToSend, messagesReceivedWithoutRecipient, environmentStep.messagesSentByTheNodes);
+
+                assert NodeNext(seqNodeStates[node][i], messagesReceivedWithoutRecipient, seqNodeStates[node][i+1], environmentStep.messagesSentByTheNodes);
+
+            }  
+            else
+            {
+                assert node in byzNodes;
+                var stepsTakenByNodeSoFar := getStepsTakeByAversarySoFar(seqNodes, byzNodes, i);
+                lemmaGetStepsTakeByAdversarySoFar(seqNodes, byzNodes, i);
+                var stepsTakenByNodeSoFarPlusOne := getStepsTakeByAversarySoFar(seqNodes, byzNodes, i + 1);
+                assert stepsTakenByNodeSoFar + 1 == stepsTakenByNodeSoFarPlusOne;
+                var adversaryBehaviour := dsBehaviour.adversaryBehaviour;
+                // var seqAdvStates := adversaryBehaviour.steps;
+                var step := adversaryBehaviour.steps[stepsTakenByNodeSoFar];
+
+
+
+                assert AdversaryNext(seqAdvStates[i], step.messageReceived, seqAdvStates[i+1], step.messagesToSend);
+
+                assert AdversaryNext(s.adversary, step.messageReceived, s'.adversary, step.messagesToSend);
+
+                lemmajkfladjklfaHelper5(s.adversary, step.messageReceived, s'.adversary, step.messagesToSend, messagesReceivedWithoutRecipient, environmentStep.messagesSentByTheNodes);
+
+                assert AdversaryNext(s.adversary, messagesReceivedWithoutRecipient, s'.adversary, environmentStep.messagesSentByTheNodes);
+
+                forall node' | node' in allNodes 
+                ensures seqNodeStates[node'][i] == seqNodeStates[node'][i+1];
+                {
+                    // assert 
+                    // lemmaGetSeqHonestNodeStates(dsBehaviour, configuration, node', seqNodes, seqNodeStates[node']);
+                    // assert seqNodeStates[node'][i] == seqNodeStates[node'][i+1];
+
+                    if node' in honestNodes
+                    {
+                        assert seqNodes[i] != node';
+
+                        assert node' in allNodes;
+                        assert pGetSeqHonestNodeStatesHelper(dsBehaviour.nodesBehaviours[node'], seqNodes, seqNodeStates[node'], node', i);
+                        assert seqNodeStates[node'][i] == seqNodeStates[node'][i+1];
+                    }
+                    else
+                    {
+                        assert seqNodeStates[node'][i] == seqNodeStates[node'][i+1];
+                    }
+
+                }                 
+
+                lemmajkfladjklfaHelper4(s, s', allNodes);
+
+                assert s.nodes == s'.nodes;
+
+                // assert step.messagesToSend == environmentStep.messagesSentByTheNodes;
+
+                // assert AdversaryNext(seqAdvStates[i], step.messageReceived, seqAdvStates[i+1], step.messagesToSend)
+            } 
+
+            assert forall n | n in honestNodes :: validNodeState(seqNodeStates[n][i]);
+            // lemmaGetSeqHonestNodeStates2(dsBehaviour, configuration, )
+
+            // forall node': Address | node' in honestNodes
+            // {
+            //     // var QbftNodeBehaviour := dsBehaviour.nodesBehaviours[node'];
+            //     // assert pGetSeqHonestNodeStatesHelper(QbftNodeBehaviour, seqNodes, seqNodeStates[node'], node', i);
+
+            //     // assert validNodeState(seqNodeStates[node'][i]);
+            //     lemmaGetSeqHonestNodeStates2(dsBehaviour, configuration, node', seqNodes, seqNodeStates[node'], i);
+            // }
+
+            // assert
+            // && NetworkNext(s.environment,s'.environment,environmentStep.messagesSentByTheNodes,environmentStep.messagesReceivedByTheNodes)
+            // && (forall mr:QbftMessageWithRecipient | mr in environmentStep.messagesReceivedByTheNodes :: mr.recipient == node)
+            // && var messageReceived := set mr:QbftMessageWithRecipient | mr in environmentStep.messagesReceivedByTheNodes :: mr.message;
+            // && node in s.nodes
+            // && s'.nodes.Keys == s.nodes.Keys
+            // && (
+            //     if isHonest(s,node) then
+            //         && s'.nodes == s.nodes[node := s'.nodes[node]]
+            //         && s'.adversary == s.adversary
+            //         && NodeNext(s.nodes[node],messageReceived,s'.nodes[node],environmentStep.messagesSentByTheNodes)
+            //     else
+            //         && s'.nodes == s.nodes
+            //         && AdversaryNext(s.adversary,messageReceived,s'.adversary,environmentStep.messagesSentByTheNodes)
+            // )
+            // && s'.configuration == s.configuration  
+            // ;          
+
+            assert DSNextNode(s, s', environmentStep.messagesSentByTheNodes, environmentStep.messagesReceivedByTheNodes, node);
+        }
+
+        forall n, i:nat | n in honestNodes 
+        ensures pLemmaGetSeqHonestNodeStates3ForAll2(dsBehaviour, n, seqNodes, dsStates[i].nodes[n], i);
+        {
+            assert pLemmaGetSeqHonestNodeStates3ForAll(dsBehaviour, n, seqNodes, seqNodeStates[n], i);
+            assert pLemmaGetSeqHonestNodeStates3ForAll2(dsBehaviour, n, seqNodes, seqNodeStates[n][i], i);
+            assert pLemmaGetSeqHonestNodeStates3ForAll2(dsBehaviour, n, seqNodes, dsStates[i].nodes[n], i);
+            // assert 
+            // lemmaGetSeqHonestNodeStates3ForAll(dsBehaviour, configuration, n, seqNodes, seqNodeStates[n]);
+        }        
+
+        forall n | n in honestNodes 
+        ensures 
+            if pGetStepsTakeByNodeSoFarIsLimited(seqNodes, n) then
+                forall i: nat | i + 1 <= getMaxWhenGetStepsTakeByNodeSoFarIsLimited(seqNodes, n).1 :: pLemmaGetSeqHonestNodeStates4ForAll2(dsBehaviour, n, seqNodes, dsStates, i) 
+            else
+                forall i: nat :: pLemmaGetSeqHonestNodeStates4ForAll2(dsBehaviour, n, seqNodes, dsStates, i)  
+        {
+            if !pGetStepsTakeByNodeSoFarIsLimited(seqNodes, n)
+            {
+                forall i: nat
+                ensures pLemmaGetSeqHonestNodeStates4ForAll2(dsBehaviour, n, seqNodes, dsStates, i);
+                {
+                    assert seqNodeStates[n][i] == dsStates[i].nodes[n];
+
+                    // assert forall i: nat :: pLemmaGetSeqHonestNodeStates4ForAll(dsBehaviour, n, seqNodes, seqNodeStates[n], i);
+                    assert pLemmaGetSeqHonestNodeStates4ForAll(dsBehaviour, n, seqNodes, seqNodeStates[n], i);
+                    assert pLemmaGetSeqHonestNodeStates4ForAll2(dsBehaviour, n, seqNodes, dsStates, i);
+                }
+
+            }
+            else
+            {
+                forall i: nat | i + 1 <= getMaxWhenGetStepsTakeByNodeSoFarIsLimited(seqNodes, n).1
+                ensures pLemmaGetSeqHonestNodeStates4ForAll2(dsBehaviour, n, seqNodes, dsStates, i);
+                {
+                    assert seqNodeStates[n][i] == dsStates[i].nodes[n];
+
+                    // assert forall i: nat :: pLemmaGetSeqHonestNodeStates4ForAll(dsBehaviour, n, seqNodes, seqNodeStates[n], i);
+                    assert pLemmaGetSeqHonestNodeStates4ForAll(dsBehaviour, n, seqNodes, seqNodeStates[n], i);
+                    assert pLemmaGetSeqHonestNodeStates4ForAll2(dsBehaviour, n, seqNodes, dsStates, i);
+                }
+            }
+        }        
+        // // assert dsStates
+
+        
+    }
+
+
+
+    lemma lemmajkfladjklfa2 (
+       dsBehaviour: DSBehaviour,
+       configuration: Configuration
+    ) returns (seqNodes: iseq<Address>, dsStates: iseq<DSState>)
+    requires IsValidConfiguration(configuration)
+    requires dsBehaviour in DSSpecificationBuilder(configuration).behaviours
+    requires  |validators([configuration.genesisBlock])| > 0
+    ensures forall i: nat :: dsBehaviour.nodesBehaviours.Keys <= dsStates[i].nodes.Keys
+    // ensures forall n, i:nat | n in dsBehaviour.nodesBehaviours.Keys :: pLemmaGetSeqHonestNodeStates3ForAll2(dsBehaviour, n, seqNodes, dsStates[i].nodes[n], i);
+    // ensures forall i: nat :: validDSState(dsStates[i]);
+    // ensures forall i: nat :: seqNodes[i] in dsStates[i].nodes
+    // ensures 
+            // forall i: nat :: pLemmajkfladjklfa(dsStates, seqNodes, dsBehaviour.environmentBehaviour, i)
+    //                 var environmentStep := dsBehaviour.environmentBehaviour.steps[i];
+    //                 && validDSState(dsStates[i])
+    //                 && DSNextNode(dsStates[i], dsStates[i+1], environmentStep.messagesSentByTheNodes, environmentStep.messagesReceivedByTheNodes, seqNodes[i]);  
+    // ensures forall n | n in dsBehaviour.nodesBehaviours.Keys ::
+    //         if pGetStepsTakeByNodeSoFarIsLimited(seqNodes, n) then
+    //             forall i: nat | i + 1 <= getMaxWhenGetStepsTakeByNodeSoFarIsLimited(seqNodes, n).1 :: pLemmaGetSeqHonestNodeStates4ForAll2(dsBehaviour, n, seqNodes, dsStates, i) 
+    //         else
+    //             forall i: nat :: pLemmaGetSeqHonestNodeStates4ForAll2(dsBehaviour, n, seqNodes, dsStates, i)        
+    {
+        var allNodes := seqToSet(configuration.nodes);
+        var honestNodes := dsBehaviour.nodesBehaviours.Keys;
+        var byzNodes := allNodes - honestNodes;
+       
+        seqNodes := lemmajkfladjklfaGetSeqNodes(dsBehaviour, configuration, allNodes);
+             
+
+        var seqAdvStates := lemmajkfladjklfaGetAdvStates(dsBehaviour, configuration, allNodes, seqNodes);
+
+        var seqEnvStates := lemmajkfladjklfaGetEnvStates(dsBehaviour, configuration);           
+
+        var seqNodeStates := lemmajkfladjklfaGetSeqNodeStates(dsBehaviour, configuration, allNodes, honestNodes, seqNodes);
+
+        dsStates := lemmajkfladjklfaGetDsStates(
+            configuration,
+            seqEnvStates,
+            seqNodeStates,
+            seqAdvStates,
+            allNodes
+        );
+
+        forall n, i:nat //| n in honestNodes
+        ensures isHonest(dsStates[i], n) <==> n in honestNodes
+        {
+            if n in honestNodes
+            {
+                assert n in dsStates[i].nodes;
+                assert n !in seqAdvStates[0].byz;
+                assert n !in seqAdvStates[i].byz;
+                assert isHonest(dsStates[i], n);
+            }
+
+            if isHonest(dsStates[i], n)
+            {
+                assert n in honestNodes;
+            }
+        }
+        
+        // assert forall i: nat, n: Address :: (isHonest(dsStates[i], n) ==> n in honestNodes);
+        // assert forall i: nat, n: Address :: (isHonest(dsStates[i], n) <== n in honestNodes);
+
+        // forall n | n in honestNodes 
+        // ensures 
+        //     if pGetStepsTakeByNodeSoFarIsLimited(seqNodes, n) then
+        //         forall i: nat | i + 1 <= getMaxWhenGetStepsTakeByNodeSoFarIsLimited(seqNodes, n).1 :: pLemmaGetSeqHonestNodeStates4ForAll2(dsBehaviour, n, seqNodes, dsStates, i) 
+        //     else
+        //         forall i: nat :: pLemmaGetSeqHonestNodeStates4ForAll2(dsBehaviour, n, seqNodes, dsStates, i)  
+        // {
+        //     if !pGetStepsTakeByNodeSoFarIsLimited(seqNodes, n)
+        //     {
+        //         forall i: nat
+        //         ensures pLemmaGetSeqHonestNodeStates4ForAll2(dsBehaviour, n, seqNodes, dsStates, i);
+        //         {
+        //             assert seqNodeStates[n][i] == dsStates[i].nodes[n];
+
+        //             // assert forall i: nat :: pLemmaGetSeqHonestNodeStates4ForAll(dsBehaviour, n, seqNodes, seqNodeStates[n], i);
+        //             assert pLemmaGetSeqHonestNodeStates4ForAll(dsBehaviour, n, seqNodes, seqNodeStates[n], i);
+        //             assert pLemmaGetSeqHonestNodeStates4ForAll2(dsBehaviour, n, seqNodes, dsStates, i);
+        //         }
+
+        //     }
+        //     else
+        //     {
+        //         forall i: nat | i + 1 <= getMaxWhenGetStepsTakeByNodeSoFarIsLimited(seqNodes, n).1
+        //         ensures pLemmaGetSeqHonestNodeStates4ForAll2(dsBehaviour, n, seqNodes, dsStates, i);
+        //         {
+        //             assert seqNodeStates[n][i] == dsStates[i].nodes[n];
+
+        //             // assert forall i: nat :: pLemmaGetSeqHonestNodeStates4ForAll(dsBehaviour, n, seqNodes, seqNodeStates[n], i);
+        //             assert pLemmaGetSeqHonestNodeStates4ForAll(dsBehaviour, n, seqNodes, seqNodeStates[n], i);
+        //             assert pLemmaGetSeqHonestNodeStates4ForAll2(dsBehaviour, n, seqNodes, dsStates, i);
+        //         }
+        //     }
+        // }
+    }    
+
 }
 
