dafny/ver/L1/theorems.dfy
@@ -5,6 +5,8 @@ include "support_lemmas/trace_defs.dfy"
 include "support_lemmas/trace_instrumented_lemmas.dfy"
 include "support_lemmas/trace_general_lemmas.dfy"
 include "theorems_defs.dfy"
+include "../../spec/L1/node_auxiliary_functions.dfy"
+include "distr_system_spec/common_functions.dfy"
 
 
 module L1_Theorems {
@@ -15,6 +17,9 @@ module L1_Theorems {
     import opened L1_TraceInstrumentedLemmas
     import opened L1_TraceGeneralLemmas    
     import opened L1_TheoremsDefs
+    import opened L1_AuxiliaryFunctionsAndLemmas
+    import opened L1_CommonFunctions
+
 
 
     predicate consistency(t: Trace)
@@ -65,5 +70,348 @@ module L1_Theorems {
         }
         lemmaPredicateThatHoldsForAllTracesExtractedFromValidInstrTracesAlsoHoldsForAValidTrace(c,t,consistencyAndStability);
     }  
+
+    predicate pNodeStepIndexIsWithinBounds(
+        seqNodes: iseq<Address>,
+        n: Address,
+        i: nat
+    )
+    {
+        &&  if pGetStepsTakeByNodeSoFarIsLimited(seqNodes, n) then
+                i <= getMaxWhenGetStepsTakeByNodeSoFarIsLimited(seqNodes, n).1
+            else 
+                true
+    }
+
+    lemma lemmaAHelper(
+        bc1: Blockchain,
+        bc2: Blockchain,
+        bc3: Blockchain,
+        bc4: Blockchain
+    )
+    requires consistentBlockchains(bc1, bc2)
+    requires bc1 == bc3 || bc3 == bc1 
+    requires bc2 == bc4 || bc4 == bc2 
+    ensures consistentBlockchains(bc3, bc4)
+    {  }
+
+
+    lemma lemmaAHelper2(
+        dsBehaviour: DSBehaviour,
+        dsStates: iseq<DSState>,
+        seqNodes: iseq<Address>,
+        blockchainSeqs: map<Address, iseq<Blockchain>>,
+        i: nat,
+        n1: Address
+
+    ) returns (inv1: nat)
+    requires n1 in blockchainSeqs
+    requires n1 in dsBehaviour.nodesBehaviours
+    requires blockchainSeqs == getBlockchainsSeq(dsBehaviour);
+    requires pNodeStepIndexIsWithinBounds(seqNodes, n1, i)
+    requires forall n | n in dsBehaviour.nodesBehaviours.Keys ::
+            if pGetStepsTakeByNodeSoFarIsLimited(seqNodes, n) then
+                forall i: nat | i + 1 <= getMaxWhenGetStepsTakeByNodeSoFarIsLimited(seqNodes, n).1 :: pLemmaGetSeqHonestNodeStates4ForAll2(dsBehaviour, n, seqNodes, dsStates, i) 
+            else
+                forall i: nat :: pLemmaGetSeqHonestNodeStates4ForAll2(dsBehaviour, n, seqNodes, dsStates, i) 
+    requires forall i: nat :: dsBehaviour.nodesBehaviours.Keys <= dsStates[i].nodes.Keys                
+    requires forall n | n in dsBehaviour.nodesBehaviours.Keys  ::
+        (dsStates[0].nodes[n].blockchain == dsBehaviour.nodesBehaviours[n].initialBlockchain)      
+    ensures blockchainSeqs[n1][i] == dsStates[inv1].nodes[n1].blockchain;                  
+    {
+        // var inv1: nat;
+        if i > 0 
+        {
+            var prevI: nat := i - 1;
+            if pGetStepsTakeByNodeSoFarIsLimited(seqNodes, n1) 
+            {
+                assert prevI + 1 <= getMaxWhenGetStepsTakeByNodeSoFarIsLimited(seqNodes, n1).1;
+                assert pLemmaGetSeqHonestNodeStates4ForAll2(dsBehaviour, n1, seqNodes, dsStates, prevI);
+            }
+            else
+            {
+                assert pLemmaGetSeqHonestNodeStates4ForAll2(dsBehaviour, n1, seqNodes, dsStates, prevI);
+            }
+
+            inv1 := getStepsTakeByNodeSoFarReverse(seqNodes, n1, prevI + 1);
+            assert dsBehaviour.nodesBehaviours[n1].steps[prevI].newBlockchain == dsStates[inv1].nodes[n1].blockchain;         
+
+            // assert blockchainSeqs[n1][i] == dsBehaviour.nodesBehaviours[n1].steps[i-1].newBlockchain; //
+            
+            // assert blockchainSeqs[n1][i] == dsStates[inv1].nodes[n1].blockchain;
+
+            lemmaGetBlockchainsSeq2(dsBehaviour, blockchainSeqs, n1, i);
+
+            calc == {
+                blockchainSeqs[n1][i];
+                dsBehaviour.nodesBehaviours[n1].steps[i-1].newBlockchain;
+                calc == {
+                    i - 1;
+                    prevI;
+                }
+                dsBehaviour.nodesBehaviours[n1].steps[prevI].newBlockchain;
+                dsStates[inv1].nodes[n1].blockchain;
+            }
+
+            assert blockchainSeqs[n1][i] == dsStates[inv1].nodes[n1].blockchain;
+
+         
+        }
+        else 
+        {
+            inv1 := 0;
+            assert blockchainSeqs[n1][i] == dsStates[inv1].nodes[n1].blockchain;
+        }
+        // assert blockchainSeqs[n1][i] == dsStates[inv1].nodes[n1].blockchain;        
+    }
+
+    function getBlockchainsSeq(
+        dsBehaviour: DSBehaviour
+    ): (ret: map<Address, iseq<Blockchain>>)
+    {
+        var ret := map n: Address | 
+            && n in dsBehaviour.nodesBehaviours.Keys
+            ::
+            (imap i: nat :: 
+                if i == 0 then
+                    dsBehaviour.nodesBehaviours[n].initialBlockchain
+                else
+                    dsBehaviour.nodesBehaviours[n].steps[i-1].newBlockchain
+            );
+        assert forall n | n in ret :: forall i:nat :: i in ret[n];
+        ret
+    }
+
+    lemma lemmaGetBlockchainsSeq(
+        dsBehaviour: DSBehaviour,
+        blockchainSeqs: map<Address, iseq<Blockchain>>
+    )
+    requires blockchainSeqs == getBlockchainsSeq(dsBehaviour);
+    ensures blockchainSeqs.Keys == dsBehaviour.nodesBehaviours.Keys
+    ensures forall n, i:nat | n in dsBehaviour.nodesBehaviours.Keys && i > 0:: blockchainSeqs[n][i] == dsBehaviour.nodesBehaviours[n].steps[i-1].newBlockchain
+    {
+
+    }
+
+
+    lemma lemmaGetBlockchainsSeq2(
+        dsBehaviour: DSBehaviour,
+        blockchainSeqs: map<Address, iseq<Blockchain>>,
+        n: Address,
+        i: nat
+    )
+    requires blockchainSeqs == getBlockchainsSeq(dsBehaviour);
+    requires i > 0
+    requires n in dsBehaviour.nodesBehaviours.Keys 
+    ensures blockchainSeqs.Keys == dsBehaviour.nodesBehaviours.Keys
+    ensures blockchainSeqs[n][i] == dsBehaviour.nodesBehaviours[n].steps[i-1].newBlockchain
+    {
+        lemmaGetBlockchainsSeq(dsBehaviour, blockchainSeqs);
+    }    
+
+    predicate consistencyAndStability2(
+        dsBehaviour: DSBehaviour,
+        configuration: Configuration
+    )
+    requires IsValidConfiguration(configuration)
+    requires dsBehaviour in DSSpecificationBuilder(configuration).behaviours
+    requires  |validators([configuration.genesisBlock])| > 0        
+    {
+        var blockchainSeqs := getBlockchainsSeq(dsBehaviour); 
+        var allNodes := seqToSet(configuration.nodes);
+        forall seqNodes, i:nat, j:nat, n1, n2 |
+                    && pLemmajkfladjklfaGetSeqNodes(dsBehaviour, allNodes, seqNodes)
+                    && n1 in dsBehaviour.nodesBehaviours.Keys
+                    && n2 in dsBehaviour.nodesBehaviours.Keys
+                    && pNodeStepIndexIsWithinBounds(seqNodes, n1, i)
+                    && pNodeStepIndexIsWithinBounds(seqNodes, n2, j)
+            ::
+                consistentBlockchains(
+                    blockchainSeqs[n1][i],
+                    blockchainSeqs[n2][j]
+                )
+
+    }  
+
+    lemma lemmaAHelper3(
+        dsBehaviour: DSBehaviour,
+        dsStates: iseq<DSState>,
+        seqNodes: iseq<Address>,
+        configuration: Configuration
+    ) returns (t: Trace)
+    requires DSInit(dsStates[0], configuration)
+    requires 
+            forall i: nat :: pLemmajkfladjklfa(dsStates, seqNodes, dsBehaviour.environmentBehaviour, i)   
+    ensures  validTrace(t, configuration);
+    ensures forall i: nat :: t(i) == dsStates[i]
+    {
+        forall i: nat
+        ensures 
+                    var s := dsStates[i];
+                    var s' := dsStates[i+1];        
+                    && validDSState(s)
+                    && DSNext(s, s')   
+        {
+            assert pLemmajkfladjklfa(dsStates, seqNodes, dsBehaviour.environmentBehaviour, i);
+            var s := dsStates[i];
+            var s' := dsStates[i+1];
+
+            assert validDSState(s);
+            assert DSNext(s, s');
+            // assert DSNext(dsStates[i], dsStates[i+1]);
+        }
+
+        t := 
+            (i: nat) => 
+                dsStates[i];
+
+        assert DSInit(t(0), configuration);
+
+        forall i:nat 
+        ensures 
+            && validDSState(t(i))
+            && DSNext(t(i), t(i+1))         
+        {
+            var s := t(i);
+            var s' := t(i+1);
+
+            assert s == dsStates[i];
+            assert s' == dsStates[i+1];
+
+            assert validDSState(s);
+            assert DSNext(s, s');            
+        }
+    }   
+
+    lemma lemmaA (
+       dsBehaviour: DSBehaviour,
+       configuration: Configuration
+    ) 
+    requires IsValidConfiguration(configuration)
+    requires dsBehaviour in DSSpecificationBuilder(configuration).behaviours
+    requires  |validators([configuration.genesisBlock])| > 0   
+    ensures consistencyAndStability2(dsBehaviour, configuration) 
+    {
+
+
+        var allNodes := seqToSet(configuration.nodes);
+        forall seqNodes, i:nat, j:nat, n1, n2 |
+                    && pLemmajkfladjklfaGetSeqNodes(dsBehaviour, allNodes, seqNodes)
+                    && n1 in dsBehaviour.nodesBehaviours.Keys
+                    && n2 in dsBehaviour.nodesBehaviours.Keys
+                    && pNodeStepIndexIsWithinBounds(seqNodes, n1, i)
+                    && pNodeStepIndexIsWithinBounds(seqNodes, n2, j)
+        ensures var blockchainSeqs := getBlockchainsSeq(dsBehaviour); 
+                consistentBlockchains(
+                    blockchainSeqs[n1][i],
+                    blockchainSeqs[n2][j]
+                );
+        {
+            var dsStates := lemmajkfladjklfa(dsBehaviour, configuration, seqNodes);
+
+            // forall i: nat
+            // ensures 
+            //             var s := dsStates[i];
+            //             var s' := dsStates[i+1];        
+            //             && validDSState(s)
+            //             && DSNext(s, s')   
+            // {
+            //     assert pLemmajkfladjklfa(dsStates, seqNodes, dsBehaviour.environmentBehaviour, i);
+            //     var s := dsStates[i];
+            //     var s' := dsStates[i+1];
+
+            //     assert validDSState(s);
+            //     assert DSNext(s, s');
+            //     // assert DSNext(dsStates[i], dsStates[i+1]);
+            // }
+
+            // var t: Trace := 
+            //     (i: nat) => 
+            //         dsStates[i];
+
+            // assert DSInit(t(0), configuration);
+
+            // forall i:nat 
+            // // ensures 
+            // //     && validDSState(t(i))
+            // //     && DSNext(t(i), t(i+1))         
+            // {
+            //     var s := t(i);
+            //     var s' := t(i+1);
+
+            //     assert s == dsStates[i];
+            //     assert s' == dsStates[i+1];
+
+            //     assert validDSState(s);
+            //     assert DSNext(s, s');            
+            // }
+
+            var t := lemmaAHelper3(dsBehaviour, dsStates, seqNodes, configuration);
+
+            
+
+            assert validTrace(t, configuration);
+
+            lemmaConsistencyAndStability(t, configuration);
+
+            var blockchainSeqs := getBlockchainsSeq(dsBehaviour);
+
+            assert n1 in dsBehaviour.nodesBehaviours.Keys;
+            assert n2 in dsBehaviour.nodesBehaviours.Keys;
+
+           
+            var inv1 := lemmaAHelper2(dsBehaviour, dsStates, seqNodes, blockchainSeqs, i, n1);
+            var inv2 := lemmaAHelper2(dsBehaviour, dsStates, seqNodes, blockchainSeqs, j, n2);
+
+
+
+            assert dsStates[0].nodes[n1].blockchain == [configuration.genesisBlock] == dsBehaviour.nodesBehaviours[n1].initialBlockchain;
+
+            // assert dsStates[0].nodes[n1].blockchain == dsBehaviour.nodesBehaviours[n1].initialBlockchain;
+
+            // if pGetStepsTakeByNodeSoFarIsLimited(seqNodes, n1) 
+            // {
+            //     assert i + 1 <= getMaxWhenGetStepsTakeByNodeSoFarIsLimited(seqNodes, n1).1;
+            //     assert pLemmaGetSeqHonestNodeStates4ForAll2(dsBehaviour, n1, seqNodes, dsStates, i);
+            // }
+            // else
+            // {
+            //     assert pLemmaGetSeqHonestNodeStates4ForAll2(dsBehaviour, n1, seqNodes, dsStates, i);
+            // }
+
+            // var inv1 := getStepsTakeByNodeSoFarReverse(seqNodes, n1, i + 1);
+            // assert dsBehaviour.nodesBehaviours[n1].steps[i].newBlockchain == dsStates[inv1].nodes[n1].blockchain;
+
+            // assert dsStates[inv1].nodes[n1].blockchain == dsBehaviour.nodesBehaviours[n1].steps[i].newBlockchain;
+
+            // if pGetStepsTakeByNodeSoFarIsLimited(seqNodes, n2) 
+            // {
+            //     assert j + 1 <= getMaxWhenGetStepsTakeByNodeSoFarIsLimited(seqNodes, n2).1;
+            //     assert pLemmaGetSeqHonestNodeStates4ForAll2(dsBehaviour, n2, seqNodes, dsStates, j);
+            // }
+            // else
+            // {
+            //     assert pLemmaGetSeqHonestNodeStates4ForAll2(dsBehaviour, n2, seqNodes, dsStates, j);
+            // }
+
+            // var inv2 := getStepsTakeByNodeSoFarReverse(seqNodes, n2, j + 1);
+            // assert dsBehaviour.nodesBehaviours[n2].steps[j].newBlockchain == dsStates[inv2].nodes[n2].blockchain;    
+
+            assert isHonest(t(inv1), n1);
+            assert isHonest(t(inv2), n2);        
+
+            lemmaAHelper(
+                dsStates[inv1].nodes[n1].blockchain,
+                dsStates[inv2].nodes[n2].blockchain,
+                blockchainSeqs[n1][i],
+                blockchainSeqs[n2][j]
+            );
+
+            // assert consistentBlockchains(
+            //     blockchainSeqs[n1][i],
+            //     blockchainSeqs[n2][j]
+            // );
+        }
+    }
 
 }
